WiP: major refactoring of CertGraphInit

src/cert_graph/CertGraphInit.v
@@ -150,852 +150,1417 @@ Lemma rstG_fair G T S thread (FAIR: mem_fair G):
 Proof.
   unfold rstG. by apply restrict_fair.
   (* Qed. *)
-Admitted. 
+Admitted.
 
-Lemma cert_graph_init Gf sc T S PC f_to f_from thread
-      (WF : Wf Gf)
-      (IMMCON : imm_consistent Gf sc)
-      (SIMREL : simrel_thread Gf sc PC T S f_to f_from thread sim_normal)
-      (FAIRf: mem_fair Gf)
-  :
-  exists G' sc' T' S',
-    ⟪ WF : Wf G' ⟫ /\
-    ⟪ IMMCON : imm_consistent G' sc' ⟫ /\
-    ⟪ NTID  : NTid_ thread ∩₁ G'.(acts_set) ⊆₁ covered T' ⟫ /\
-    ⟪ SIMREL : simrel_thread G' sc' PC T' S' f_to f_from thread sim_certification ⟫.
-Proof using All.
-assert (exists G, G = rstG Gf T S thread) by eauto; desc.
-forward eapply (rstG_fair) as FAIR; cycle 1; [rewrite <- H in FAIR| done]. 
+Section CertGraphInit.
+  Variable (Gf: execution) (sc: relation actid) (T: trav_config) (S: actid -> Prop).
+  Variable (PC: Configuration.Configuration.t). 
+  Variable (f_to f_from: actid -> Time.Time.t). 
+  Variable (thread: thread_id).
 
-assert (WF_SC: wf_sc Gf sc).
-by apply IMMCON.
+  Hypothesis (WF: Wf Gf).
+  Hypothesis (FAIRf: mem_fair Gf).
+  Hypothesis (IMMCON : imm_consistent Gf sc).
+  Hypothesis (SIMREL : simrel_thread Gf sc PC T S f_to f_from thread sim_normal).
+  
+  Definition G := rstG Gf T S thread.
+  Definition Gsc := ⦗E0 Gf T S thread⦘ ⨾ sc ⨾ ⦗E0 Gf T S thread⦘. 
 
-assert (ETCCOH: etc_coherent Gf sc (mkETC T S)).
-{ by cdes SIMREL; cdes COMMON. }
-assert (TCCOH: tc_coherent Gf sc T) by apply ETCCOH.
+  Lemma FAIR: mem_fair G.
+  Proof using FAIRf. forward eapply (rstG_fair); eauto. Qed.
 
-assert (RELCOV: (fun a : actid => is_w (lab Gf) a) ∩₁ (fun a : actid => is_rel (lab Gf) a) ∩₁ issued T
-⊆₁ covered T).
-by cdes SIMREL; cdes COMMON.
+  Lemma WF_SC: wf_sc Gf sc. 
+  Proof using IMMCON. by apply IMMCON. Qed.
 
-remember (⦗E0 Gf T S thread⦘ ⨾ sc ⨾ ⦗E0 Gf T S thread⦘) as Gsc.
-assert (SUB: sub_execution Gf G sc Gsc).
-{ unfold rstG in *; subst.
-apply restrict_sub.
-done.
-rewrite <- E_E0; eauto.
-rewrite E_E0; eauto.
-rewrite E0_in_Gf; eauto. }
+  Lemma ETCCOH: etc_coherent Gf sc (mkETC T S). 
+  Proof using SIMREL. by cdes SIMREL; cdes COMMON. Qed.
+  
+  Lemma TCCOH: tc_coherent Gf sc T.
+  Proof using SIMREL. by apply ETCCOH. Qed. 
 
-assert (WF_G: Wf G).
-by subst; eapply rstWF; edone.
+  Lemma RELCOV:
+    (fun a => is_w (lab Gf) a) ∩₁ (fun a : actid => is_rel (lab Gf) a) ∩₁ issued T
+                            ⊆₁ covered T.
+  Proof using SIMREL. by cdes SIMREL; cdes COMMON. Qed.
 
-assert (WF_SC_G: wf_sc G Gsc).
-by subst; eapply WF_SC_rst; edone.
+  Hint Resolve FAIR ETCCOH TCCOH WF_SC RELCOV: core.
 
-assert (RELCOV_G : is_w (lab G) ∩₁ is_rel (lab G) ∩₁ (issued T) ⊆₁ (covered T)).
-by rewrite (sub_W SUB), (sub_Rel SUB).
+  Lemma SUB: sub_execution Gf G sc Gsc. 
+  Proof using WF SIMREL.
+    unfold rstG in *; subst.
+    apply restrict_sub; eauto.  
+    rewrite <- E_E0; eauto. 
+    rewrite E_E0; eauto.
+    rewrite E0_in_Gf; eauto.
+  Qed. 
+    
+  Lemma WF_G: Wf G.
+  Proof using WF SIMREL. unfold G; eapply rstWF; eauto. Qed. 
 
-assert (RMWCOV : forall r w : actid, rmw Gf r w -> covered T r <-> covered T w) by apply SIMREL.
+  Lemma WF_SC_G: wf_sc G Gsc.
+  Proof using IMMCON WF SIMREL. unfold G; eapply WF_SC_rst; eauto. Qed. 
 
-assert (TCCOH_G : tc_coherent G Gsc T).
-{ subst; eapply TCCOH_rst; try edone. }
+  Lemma RELCOV_G: is_w (lab G) ∩₁ is_rel (lab G) ∩₁ (issued T) ⊆₁ (covered T).
+  Proof using IMMCON WF SIMREL.
+    rewrite (sub_W SUB), (sub_Rel SUB). eauto.  
+  Qed. 
 
-assert (TCCOH_rst_new_T : tc_coherent G Gsc (mkTC ( (covered T) ∪₁ ((acts_set G) ∩₁ NTid_ thread))  (issued T))).
-{ subst; eapply TCCOH_rst_new_T; eauto. }
+  Lemma RMWCOV: forall r w, rmw Gf r w -> covered T r <-> covered T w.
+  Proof using SIMREL. by apply SIMREL. Qed.
 
-assert (IT_new_co: (issued T) ∪₁ (acts_set G) ∩₁ is_w (lab G) ∩₁ Tid_ thread ≡₁ (acts_set G) ∩₁ is_w (lab G)).
-subst; eapply IT_new_co; edone.
+  Hint Resolve SUB WF_G WF_SC_G RELCOV_G RMWCOV: core.
 
-assert (ACYC_EXT_G: acyc_ext G Gsc).
-subst; eapply acyc_ext_rst; edone.
+  Lemma TCCOH_G: tc_coherent G Gsc T. 
+  Proof using WF IMMCON SIMREL. subst; eapply TCCOH_rst; eauto. Qed. 
 
-assert (CSC_G : coh_sc G Gsc).
-subst; eapply coh_sc_rst; edone.
+  Lemma TCCOH_rst_new_T:
+    tc_coherent G Gsc (mkTC ((covered T) ∪₁ ((acts_set G) ∩₁ NTid_ thread))  (issued T)).
+  Proof using WF SIMREL IMMCON. subst; eapply TCCOH_rst_new_T; eauto. Qed. 
 
-assert (COH_G: coherence G).
-subst; eapply coherence_rst; edone.
+  Lemma IT_new_co:
+    (issued T) ∪₁ (acts_set G) ∩₁ is_w (lab G) ∩₁ Tid_ thread ≡₁ (acts_set G) ∩₁ is_w (lab G).
+  Proof using WF SIMREL. subst; eapply IT_new_co; eauto. Qed. 
 
-assert (AT_G: rmw_atomicity G).
-subst; eapply rmw_atomicity_rst; edone.
+  Lemma ACYC_EXT_G: acyc_ext G Gsc.
+  Proof using SIMREL WF IMMCON. subst; eapply acyc_ext_rst; eauto. Qed. 
 
-assert (E_to_S: (acts_set G) ⊆₁ (covered T) ∪₁ dom_rel ((sb G)^? ⨾ ⦗S⦘)).
-subst; eapply E_to_S; edone.
+  Lemma CSC_G: coh_sc G Gsc.
+  Proof using WF SIMREL IMMCON. subst; eapply coh_sc_rst; eauto. Qed. 
 
-assert (Grfe_E : dom_rel (rfe G) ⊆₁ (issued T)).
-subst; eapply Grfe_E; edone.
+  Lemma COH_G: coherence G. 
+  Proof using WF SIMREL IMMCON. subst; eapply coherence_rst; eauto. Qed. 
 
-assert (E_F_AcqRel_in_C: (acts_set G) ∩₁ (is_f (lab G)) ∩₁ (is_ra (lab G)) ⊆₁ (covered T)).
-subst; eapply E_F_AcqRel_in_C; edone.
+  Lemma AT_G: rmw_atomicity G. 
+  Proof using WF SIMREL IMMCON. subst; eapply rmw_atomicity_rst; eauto. Qed. 
 
-assert ( COMP_ACQ: forall r (IN: ((acts_set G) ∩₁ (is_r (lab G)) ∩₁ (is_acq (lab G))) r), exists w, (rf G) w r).
-{ subst; eapply COMP_ACQ; edone. }
+  Lemma E_to_S: (acts_set G) ⊆₁ (covered T) ∪₁ dom_rel ((sb G)^? ⨾ ⦗S⦘). 
+  Proof using WF SIMREL. subst; eapply E_to_S; eauto. Qed. 
+  
+  Lemma Grfe_E : dom_rel (rfe G) ⊆₁ (issued T). 
+  Proof using WF SIMREL IMMCON. subst; eapply Grfe_E; eauto. Qed. 
 
-assert (dom_rel
-          ((rmw G ⨾ rfi G)＊ ⨾ ⦗acts_set G ∩₁ (is_r (lab G)) ∩₁
-           (is_acq (lab G))⦘) ⊆₁ codom_rel (rf G))
-  as RMW_RFI_ACQ.
-{ subst; eapply COMP_RMWRFI_ACQ; edone. }
+  Lemma E_F_AcqRel_in_C:
+    (acts_set G) ∩₁ (is_f (lab G)) ∩₁ (is_ra (lab G)) ⊆₁ (covered T).
+  Proof using WF SIMREL. subst; eapply E_F_AcqRel_in_C; eauto. Qed. 
 
-assert ( urr_helper: dom_rel (((hb G) ⨾ ⦗(is_f (lab G)) ∩₁ (is_sc (lab G))⦘)^? ⨾ Gsc^? ⨾ (hb G)^? ⨾ (release G) ⨾ ⦗(issued T)⦘) ⊆₁ (covered T)).
-subst; eapply urr_helper; edone.
+  Lemma COMP_ACQ:
+    forall r (IN: ((acts_set G) ∩₁ (is_r (lab G)) ∩₁ (is_acq (lab G))) r), exists w, (rf G) w r.
+  Proof using WF SIMREL IMMCON.  subst; eapply COMP_ACQ; eauto. Qed.
 
-assert ( urr_helper_C: dom_rel (((hb G) ⨾ ⦗(is_f (lab G)) ∩₁ (is_sc (lab G))⦘)^? ⨾ Gsc^? ⨾ (hb G)^? ⨾ ((release G) ⨾ (rf G))^? ⨾ ⦗(covered T)⦘) ⊆₁ (covered T)).
-subst; eapply urr_helper_C; edone.
+  Lemma RMW_RFI_ACQ:
+    dom_rel
+      ((rmw G ⨾ rfi G)＊ ⨾ ⦗acts_set G ∩₁ (is_r (lab G)) ∩₁ (is_acq (lab G))⦘)
+      ⊆₁ codom_rel (rf G). 
+  Proof using WF SIMREL IMMCON. subst; eapply COMP_RMWRFI_ACQ; eauto. Qed. 
 
-assert ( W_hb_sc_hb_to_I_NTid: dom_rel (⦗(is_w (lab G))⦘ ⨾ (hb G) ⨾ (Gsc ⨾ (hb G))^? ⨾ ⦗(issued T) ∩₁ NTid_ thread⦘) ⊆₁ (issued T)).
-subst; eapply W_hb_sc_hb_to_I_NTid; edone.
+  Lemma urr_helper:
+    dom_rel (((hb G) ⨾ ⦗(is_f (lab G)) ∩₁ (is_sc (lab G))⦘)^? ⨾ Gsc^? ⨾ (hb G)^? ⨾ (release G) ⨾ ⦗(issued T)⦘) ⊆₁ (covered T). 
+  Proof using WF SIMREL IMMCON. subst; eapply urr_helper; eauto. Qed. 
 
-assert ( detour_E : dom_rel ((detour G) ⨾ ⦗(acts_set G) ∩₁ NTid_ thread⦘) ⊆₁ (issued T)).
-subst; eapply detour_E; edone.
+  Lemma urr_helper_C:
+    dom_rel (((hb G) ⨾ ⦗(is_f (lab G)) ∩₁ (is_sc (lab G))⦘)^? ⨾ Gsc^? ⨾ (hb G)^? ⨾ ((release G) ⨾ (rf G))^? ⨾ ⦗(covered T)⦘) ⊆₁ (covered T). 
+  Proof using WF SIMREL IMMCON. subst; eapply urr_helper_C; eauto. Qed. 
 
-assert ( detour_Acq_E : dom_rel ((detour G) ⨾ ⦗(acts_set G) ∩₁ (is_r (lab G)) ∩₁ (is_acq (lab G))⦘) ⊆₁ (issued T)).
-subst; eapply detour_Acq_E; edone.
+  Lemma W_hb_sc_hb_to_I_NTid:
+    dom_rel (⦗(is_w (lab G))⦘ ⨾ (hb G) ⨾ (Gsc ⨾ (hb G))^? ⨾ ⦗(issued T) ∩₁ NTid_ thread⦘) ⊆₁ (issued T).
+  Proof using WF SIMREL IMMCON. subst; eapply W_hb_sc_hb_to_I_NTid; eauto. Qed.
 
-assert ( hb_sc_hb_de : ⦗((acts_set G) \₁ (covered T)) ∩₁ ((acts_set G) \₁ (issued T))⦘ ⨾ (hb G) ⨾ (Gsc ⨾ (hb G))^? ⊆ (sb G)).
-subst; eapply hb_sc_hb_de; edone.
+  Lemma detour_E:
+    dom_rel ((detour G) ⨾ ⦗(acts_set G) ∩₁ NTid_ thread⦘) ⊆₁ (issued T). 
+  Proof using WF SIMREL. subst; eapply detour_E; eauto. Qed. 
 
-assert (COMP_C : (covered T) ∩₁ (is_r (lab G)) ⊆₁ codom_rel (rf G)).
-subst; eapply COMP_C; edone.
+  Lemma detour_Acq_E:
+    dom_rel ((detour G) ⨾ ⦗(acts_set G) ∩₁ (is_r (lab G)) ∩₁ (is_acq (lab G))⦘) ⊆₁ (issued T).
+  Proof using WF SIMREL. subst; eapply detour_Acq_E; eauto. Qed.
 
-assert (COMP_NTID : (acts_set G) ∩₁ NTid_ thread ∩₁ (is_r (lab G)) ⊆₁ codom_rel (rf G)).
-subst; eapply COMP_NTID; edone.
+  Lemma hb_sc_hb_de:
+    ⦗((acts_set G) \₁ (covered T)) ∩₁ ((acts_set G) \₁ (issued T))⦘ ⨾ (hb G) ⨾ (Gsc ⨾ (hb G))^? ⊆ (sb G).
+  Proof using WF SIMREL IMMCON. subst; eapply hb_sc_hb_de; eauto. Qed. 
 
-assert (COMP_PPO : dom_rel ((ppo G) ⨾ ⦗(issued T)⦘) ∩₁ (is_r (lab G)) ⊆₁ codom_rel (rf G)).
-{ subst; eapply COMP_PPO; edone. }
-assert (COM_PPO_ALT : dom_rel (ppo G ⨾ ⦗issued T⦘) ⊆₁ codom_rel (rf G)).
-{ rewrite (dom_l (wf_ppoD G)), !seqA.
-  rewrite dom_eqv1. by rewrite set_interC. }
+  Hint Resolve TCCOH_G TCCOH_rst_new_T IT_new_co ACYC_EXT_G CSC_G COH_G: core.
+  Hint Resolve AT_G E_to_S Grfe_E E_F_AcqRel_in_C COMP_ACQ RMW_RFI_ACQ: core.
+  Hint Resolve urr_helper urr_helper_C W_hb_sc_hb_to_I_NTid detour_E detour_Acq_E hb_sc_hb_de: core.
 
-assert (acts_G_in_acts_Gf : acts_set G ⊆₁ acts_set Gf).
-by apply (sub_E_in SUB).
+  Lemma COMP_C: (covered T) ∩₁ (is_r (lab G)) ⊆₁ codom_rel (rf G).
+  Proof using WF SIMREL IMMCON. subst; eapply COMP_C; eauto. Qed. 
 
-assert (lab_G_eq_lab_Gf : lab G = lab Gf).
-{ rewrite H. unfold rstG. by unfold restrict. }
+  Lemma COMP_NTID:
+    (acts_set G) ∩₁ NTid_ thread ∩₁ (is_r (lab G)) ⊆₁ codom_rel (rf G).
+  Proof using WF SIMREL IMMCON. subst; eapply COMP_NTID; eauto. Qed. 
 
-assert (rmw_G_rmw_Gf : rmw G ≡
-                       ⦗ E0 Gf T S thread ⦘ ⨾ rmw Gf ⨾ ⦗ E0 Gf T S thread ⦘).
-{ rewrite H. unfold rstG. by unfold restrict. }
+  Lemma COMP_PPO:
+    dom_rel ((ppo G) ⨾ ⦗(issued T)⦘) ∩₁ (is_r (lab G)) ⊆₁ codom_rel (rf G).
+  Proof using WF SIMREL IMMCON. subst; eapply COMP_PPO; eauto. Qed.
 
-cdes SIMREL. cdes LOCAL.
-red in STATE. desc.
-cdes STATE0.
+  Lemma COM_PPO_ALT: dom_rel (ppo G ⨾ ⦗issued T⦘) ⊆₁ codom_rel (rf G). 
+  Proof using WF SIMREL IMMCON.
+    rewrite (dom_l (wf_ppoD G)), !seqA.
+    rewrite dom_eqv1. rewrite set_interC. apply COMP_PPO. 
+  Qed.
 
-(* set (CT := E0 Gf T S thread ∩₁ Tid_ thread). *)
-set (CT := mkCT Gf T S thread).
-assert (CT ≡₁ (covered T ∪₁ issued T ∪₁ dom_rel ((sb Gf)^? ⨾ ⦗Tid_ thread ∩₁ S⦘))
-           ∩₁ Tid_ thread) as CTALT.
-{ subst CT. unfold mkCT.  unfold E0.
-  arewrite (rmw Gf ⨾ ⦗NTid_ thread ∩₁ issued T⦘ ≡
-            ⦗NTid_ thread⦘ ⨾ rmw Gf ⨾ ⦗NTid_ thread ∩₁ issued T⦘).
-  { split; [|basic_solver].
+  Lemma acts_G_in_acts_Gf: acts_set G ⊆₁ acts_set Gf.
+  Proof using WF SIMREL. by apply (sub_E_in SUB). Qed. 
+
+  Lemma lab_G_eq_lab_Gf: lab G = lab Gf.
+  Proof using. vauto. Qed. 
+
+  Lemma rmw_G_rmw_Gf:
+    rmw G ≡ ⦗ E0 Gf T S thread ⦘ ⨾ rmw Gf ⨾ ⦗ E0 Gf T S thread ⦘.
+  Proof using. vauto. Qed.
+
+  Hint Resolve COMP_C COMP_NTID COMP_PPO COM_PPO_ALT acts_G_in_acts_Gf lab_G_eq_lab_Gf rmw_G_rmw_Gf: core. 
+   
+  Definition CT := mkCT Gf T S thread. 
+  
+  Lemma CTALT:
+    CT ≡₁ (covered T ∪₁ issued T ∪₁ dom_rel ((sb Gf)^? ⨾ ⦗Tid_ thread ∩₁ S⦘)) ∩₁ Tid_ thread.
+  Proof using WF SIMREL. 
+    unfold CT, mkCT, E0.
+    arewrite (rmw Gf ⨾ ⦗NTid_ thread ∩₁ issued T⦘ ≡
+                  ⦗NTid_ thread⦘ ⨾ rmw Gf ⨾ ⦗NTid_ thread ∩₁ issued T⦘).
+    2: { basic_solver 10. }
+    split; [|basic_solver].
     intros x y HH. apply seq_eqv_l. split; auto.
     apply seq_eqv_r in HH. destruct HH as [RMW [AA BB]].
     intros CC. apply AA. rewrite <- CC. symmetry.
-      by apply (wf_rmwt WF). }
-  basic_solver 10. }
+      by apply (wf_rmwt WF). 
+  Qed.
 
-assert (CT ⊆₁ acts_set Gf) as CTEE.
-{ rewrite CTALT.
-  rewrite (coveredE TCCOH).
-  rewrite (issuedE TCCOH).
-  rewrite (etc_S_in_E ETCCOH).
-  rewrite wf_sbE. basic_solver. }
+  Lemma CTEE: CT ⊆₁ acts_set Gf.
+  Proof using WF SIMREL.
+    rewrite CTALT.
+    rewrite (coveredE TCCOH).
+    rewrite (issuedE TCCOH).
+    rewrite (etc_S_in_E ETCCOH).
+    rewrite wf_sbE. basic_solver.
+  Qed. 
 
-assert (CREP_weak :
-          forall e (CTE : CT e),
-               exists index : nat,
-                 ⟪ EREP : e = ThreadEvent thread index ⟫).
-{ ins. apply CTALT in CTE. destruct CTE as [AA BB].
-  destruct e; desf. simpls. eauto. }
+  Lemma CREP_weak:
+          forall e (CTE : CT e), exists index : nat,
+              ⟪ EREP : e = ThreadEvent thread index ⟫.
+  Proof using WF SIMREL.
+    ins. apply CTALT in CTE. destruct CTE as [AA BB].
+    cdes SIMREL. cdes LOCAL.
+    destruct e; desf. simpls. eauto.
+  Qed. 
 
-assert (wf_thread_state thread state') as GPC'.
-{ eapply wf_thread_state_steps; eauto. }
+  Lemma thread_ninit: thread <> tid_init.
+  Proof using SIMREL. cdes SIMREL. cdes LOCAL. auto. Qed.
 
-assert (exists ctindex,
-           ⟪ CCLOS :forall index (LT : index < ctindex),
-             CT (ThreadEvent thread index) ⟫ /\
-           ⟪ CREP : forall e (CTE : CT e),
-               exists index : nat,
-                 ⟪ EREP : e = ThreadEvent thread index ⟫ /\
-                 ⟪ ILT : index < ctindex ⟫ ⟫).
-{ destruct (classic (exists e, CT e)) as [|NCT].
-  2: { exists 0. splits.
-       { ins. inv LT. }
-       ins. exfalso. apply NCT. eauto. }
-  desc.
-  assert (acyclic (sb Gf ⨾ ⦗ CT ⦘)) as AC.
-  { arewrite (sb Gf ⨾ ⦗CT⦘ ⊆ sb Gf). apply sb_acyclic. }
-  (* set (doml := filterP CT (acts Gf)). *)
-  (* assert (forall c, (sb Gf ⨾ ⦗CT⦘)＊ e c -> In c doml) as UU. *)
-  (* { intros c SCC. apply rtE in SCC. destruct SCC as [SCC|SCC]. *)
-  (*   { red in SCC. desf. apply in_filterP_iff. split; auto. by apply CTEE. } *)
-  (*   apply inclusion_ct_seq_eqv_r in SCC. apply seq_eqv_r in SCC. *)
-  (*   apply in_filterP_iff. split; auto; [apply CTEE|]; desf. } *)
-  assert (exists doml, (forall c, (sb Gf ⨾ ⦗CT⦘)＊ e c -> In c doml)) as [doml UU].
-  { fold (set_finite ((sb Gf ⨾ ⦗CT⦘)＊ e)).
-    arewrite ((sb Gf ⨾ ⦗CT⦘)＊ e ⊆₁ codom_rel (⦗eq e⦘ ⨾ (sb Gf ⨾ ⦗CT⦘)＊)) by vauto.
+  Hint Resolve thread_ninit: core.
+
+  Lemma CTINDEX 
+        (state': Language.state (PromiseLTS.thread_lts thread))
+        (TEH: thread_restricted_execution Gf thread (ProgToExecution.G state'))
+        (GPC': wf_thread_state thread state'):
+    exists ctindex,
+      ⟪ CCLOS :forall index (LT : index < ctindex),
+          CT (ThreadEvent thread index) ⟫ /\
+      ⟪ CREP : forall e (CTE : CT e),
+          exists index : nat,
+            ⟪ EREP : e = ThreadEvent thread index ⟫ /\
+            ⟪ ILT : index < ctindex ⟫ ⟫.
+  Proof using WF SIMREL.
+    destruct (classic (exists e, CT e)) as [|NCT].
+    2: { exists 0. splits.
+         { ins. inv LT. }
+         ins. exfalso. apply NCT. eauto. }
+    desc.
+    assert (acyclic (sb Gf ⨾ ⦗ CT ⦘)) as AC.
+    { arewrite (sb Gf ⨾ ⦗CT⦘ ⊆ sb Gf). apply sb_acyclic. }
+    assert (exists doml, (forall c, (sb Gf ⨾ ⦗CT⦘)＊ e c -> In c doml)) as [doml UU].
+    { fold (set_finite ((sb Gf ⨾ ⦗CT⦘)＊ e)).
+      arewrite ((sb Gf ⨾ ⦗CT⦘)＊ e ⊆₁ codom_rel (⦗eq e⦘ ⨾ (sb Gf ⨾ ⦗CT⦘)＊)) by vauto.
     arewrite ((sb Gf ⨾ ⦗CT⦘)＊ ⊆ (sb Gf ⨾ ⦗CT⦘)^?).
     { rewrite crE, rtE. apply union_mori; [basic_solver| ].
       apply inclusion_t_ind; [basic_solver| ].
       generalize (@sb_trans Gf). basic_solver. }
     rewrite crE, seq_union_r, codom_union. apply set_finite_union. split.
     { exists [e]. basic_solver. }
-    rewrite <- seqA, codom_seq_eqv_r. 
-    subst CT. forward eapply CT_fin; eauto. }
+    rewrite <- seqA, codom_seq_eqv_r.
+    unfold CT. forward eapply CT_fin; eauto. }
     
-  edestruct (last_exists doml AC UU) as [max [MM1 MM2]].
-  
-  assert (CT max) as CTMAX.
-  { apply rtE in MM1. destruct MM1 as [MM1|MM1].
-    { red in MM1. desf. }
-    apply inclusion_ct_seq_eqv_r in MM1. apply seq_eqv_r in MM1. desf. }
-  assert (Tid_ thread max) as CTTID by apply CTMAX.
-  destruct max as [l|mthread mindex]; [by desf|].
-  simpls. rewrite CTTID in *.
-  assert (acts_set Gf (ThreadEvent thread mindex)) as EEM.
-  { by apply CTEE. }
-  exists (1 + mindex). splits.
-  { ins. apply CTALT in CTMAX.
-    apply CTALT. split; auto. 
-    apply le_lt_or_eq in LT. destruct LT as [LT|LT].
-    2: { inv LT. apply CTMAX. }
-    assert ((ProgToExecution.G state').(acts_set) (ThreadEvent thread mindex)) as PP.
-    { apply (tr_acts_set TEH). by split. }
-    assert ((acts_set Gf) (ThreadEvent thread index)) as EEE.
-    { apply (tr_acts_set TEH). eapply acts_rep in PP; eauto. desc.
-      eapply GPC'.(acts_clos). inv REP. omega. }
-    assert (sb Gf (ThreadEvent thread index) (ThreadEvent thread mindex)) as QQ.
-    { red.
-      apply seq_eqv_l. split; auto.
+    edestruct (last_exists doml AC UU) as [max [MM1 MM2]].
+    
+    assert (CT max) as CTMAX.
+    { apply rtE in MM1. destruct MM1 as [MM1|MM1].
+      { red in MM1. desf. }
+      apply inclusion_ct_seq_eqv_r in MM1. apply seq_eqv_r in MM1. desf. }
+    assert (Tid_ thread max) as CTTID by apply CTMAX.
+    destruct max as [l|mthread mindex].
+    { by destruct thread_ninit. }
+    simpls. rewrite CTTID in *.
+    assert (acts_set Gf (ThreadEvent thread mindex)) as EEM.
+    { by apply CTEE. }
+    exists (1 + mindex). splits.
+    { ins. apply CTALT in CTMAX.
+      apply CTALT. split; auto.
+      apply le_lt_or_eq in LT. destruct LT as [LT|LT].
+      2: { inv LT. apply CTMAX. }
+      assert ((ProgToExecution.G state').(acts_set) (ThreadEvent thread mindex)) as PP.
+      { apply (tr_acts_set TEH). by split. }
+      assert ((acts_set Gf) (ThreadEvent thread index)) as EEE.
+      { apply (tr_acts_set TEH). eapply acts_rep in PP; eauto.
+        desc. eapply GPC'.(acts_clos). inv REP. omega. }
+      assert (sb Gf (ThreadEvent thread index) (ThreadEvent thread mindex)) as QQ.
+      { red.
+        apply seq_eqv_l. split; auto.
+        apply seq_eqv_r. split; auto.
+        red. split; auto. omega. }
+      destruct CTMAX as [[[AA|AA]|[z AA]] _].
+      { do 2 left. apply TCCOH in AA. apply AA. eexists.
+        apply seq_eqv_r. split; eauto. }
+      { right. exists (ThreadEvent thread mindex).
+        apply seq_eqv_r. split; auto.
+        split; auto. by apply (etc_I_in_S ETCCOH). }
+      right. exists z. apply seq_eqv_r in AA. destruct AA as [AA1 AA2].
       apply seq_eqv_r. split; auto.
-      red. split; auto. omega. }
-    destruct CTMAX as [[[AA|AA]|[z AA]] _].
-    { do 2 left. apply TCCOH in AA. apply AA. eexists.
-      apply seq_eqv_r. split; eauto. }
-    { right. exists (ThreadEvent thread mindex).
-      apply seq_eqv_r. split; auto.
-      split; auto. by apply (etc_I_in_S ETCCOH). }
-    right. exists z. apply seq_eqv_r in AA. destruct AA as [AA1 AA2].
-    apply seq_eqv_r. split; auto.
-    apply rewrite_trans_seq_cr_cr.
-    { apply sb_trans. }
-    eexists; split; [|by eauto].
-      by apply r_step. }
-  ins. set (CTE' := CTE).
-  apply CREP_weak in CTE'. desc.
-  eexists. splits; eauto.
-  destruct (le_gt_dec index mindex) as [LL|LL].
-  { by apply le_lt_n_Sm. }
-  exfalso.
-  eapply MM2. apply seq_eqv_r. split; [|by apply CTE].
-  red.
-  apply seq_eqv_l. split; auto.
-  apply seq_eqv_r. split; auto.
-  red. rewrite EREP. by split. }
-desc.
+      apply rewrite_trans_seq_cr_cr.
+      { apply sb_trans. }
+      eexists; split; [|by eauto].
+        by apply r_step. }
+    ins. set (CTE' := CTE).
+    apply CREP_weak in CTE'. desc.
+    eexists. splits; eauto.
+    destruct (le_gt_dec index mindex) as [LL|LL].
+    { by apply le_lt_n_Sm. }
+    exfalso.
+    eapply MM2. apply seq_eqv_r. split; [|by apply CTE].
+    red.
+    apply seq_eqv_l. split; auto.
+    apply seq_eqv_r. split; [vauto| by apply CTEE].
+  Qed.
 
-assert (exists state'',
-           ⟪ STEPS'' : (step thread)＊ state state'' ⟫ /\
-           ⟪ TEH''   : thread_restricted_execution G thread state''.(ProgToExecution.G) ⟫).
-{ edestruct steps_middle_set with (C:=CT) (state0:=state) (state':=state')
-    as [state'']; eauto.
-  { intros x HH. apply (acts_rep GPC) in HH.
-    desc. 
+  Lemma STATE''
+        (state: ProgToExecution.state)
+        (state': Language.state (PromiseLTS.thread_lts thread))
+        (ctindex: nat)
+        (STEPS : (step thread)＊ state state')
+        (TEH: thread_restricted_execution Gf thread (ProgToExecution.G state'))
+        (GPC : wf_thread_state thread state)
+        (GPC' : wf_thread_state thread state')
+        (PCOV : forall index, covered T (ThreadEvent thread index) <-> index < eindex state)
+        (CCLOS: forall index (LT : index < ctindex), CT (ThreadEvent thread index))
+        (CREP: forall e, CT e -> exists index : nat,
+              e = ThreadEvent thread index /\ index < ctindex)
+      :
+    exists state'',
+      ⟪ STEPS'' : (step thread)＊ state state'' ⟫ /\
+      ⟪ TEH'': thread_restricted_execution G thread state''.(ProgToExecution.G) ⟫.
+  Proof using WF SIMREL.
+    edestruct steps_middle_set with (C:=CT) (state0:=state) (state':=state')
+      as [state'']; eauto.
+    { intros x HH. apply (acts_rep GPC) in HH.
+    desc.
     apply CTALT. rewrite REP in *. split; auto.
     do 2 left. by apply PCOV. }
-  { rewrite CTALT. rewrite (tr_acts_set TEH).
-    apply set_subset_inter; [|done].
-    rewrite coveredE with (G:=Gf); eauto.
-    rewrite issuedE with (G:=Gf); eauto.
-    rewrite (etc_S_in_E ETCCOH).
-    rewrite wf_sbE. basic_solver. }
-  { ins.
-    apply (tr_rmw TEH) in RMW.
-    apply seq_eqv_l in RMW. destruct RMW as [TIDR RMW].
-    apply seq_eqv_r in RMW. destruct RMW as [RMW TIDW].
-    apply (dom_l (wf_rmwD WF)) in RMW.
-    apply seq_eqv_l in RMW. destruct RMW as [RREX RMW].
-    assert (is_r (lab Gf) r) as RR by type_solver.
-    split; intros AA.
-    all: apply CTALT; split; auto.
-    all: apply CTALT in AA; destruct AA as [[[AA|AA]|AA] _].
-    1,4: do 2 left; cdes COMMON; by apply (RMWCOV r w RMW).
-    { apply (issuedW TCCOH) in AA. type_solver. }
-    { right. unfolder in AA. desf.
-      { apply (reservedW WF ETCCOH) in AA2. type_solver. }
-      exists y. apply seq_eqv_r. split; [|split]; auto.
-      destruct (classic (w = y)) as [|NEQ]; subst.
+    { rewrite CTALT. rewrite (tr_acts_set TEH).
+      apply set_subset_inter; [|done].
+      rewrite coveredE with (G:=Gf); eauto.
+      rewrite issuedE with (G:=Gf); eauto.
+      rewrite (etc_S_in_E ETCCOH).
+      rewrite wf_sbE. basic_solver. }
+    { cdes SIMREL. 
+      ins.
+      apply (tr_rmw TEH) in RMW.
+      apply seq_eqv_l in RMW. destruct RMW as [TIDR RMW].
+      apply seq_eqv_r in RMW. destruct RMW as [RMW TIDW].
+      apply (dom_l (wf_rmwD WF)) in RMW.
+      apply seq_eqv_l in RMW. destruct RMW as [RREX RMW].
+      assert (is_r (lab Gf) r) as RR by type_solver.
+      split; intros AA.
+      all: apply CTALT; split; auto.
+      all: apply CTALT in AA; destruct AA as [[[AA|AA]|AA] _].
+      1,4: do 2 left; cdes COMMON; by apply (RMWCOV r w RMW).
+      { apply (issuedW TCCOH) in AA. type_solver. }
+      { right. unfolder in AA. desf.
+        { apply (reservedW WF ETCCOH) in AA2. type_solver. }
+        exists y. apply seq_eqv_r. split; [|split]; auto.
+        destruct (classic (w = y)) as [|NEQ]; subst.
+        { basic_solver. }
+        edestruct (@sb_semi_total_l Gf r y w WF); auto.
+        { intros HH. apply (init_w WF) in HH.
+          clear -RR HH. type_solver. }
+        { by apply (rmw_in_sb WF). }
+        exfalso. eapply (wf_rmwi WF); eauto. }
+      { right. exists w. apply seq_eqv_r. split; [|split]; auto.
+        { right. by apply rmw_in_sb. }
+        apply (etc_I_in_S ETCCOH). apply AA. }
+      right. destruct AA as [y AA]. apply seq_eqv_r in AA. destruct AA as [AA BB].
+      exists y. apply seq_eqv_r. split; auto.
+      right. apply rewrite_trans_seq_cr_r.
+      { apply sb_trans. }
+      eexists; split; eauto. by apply rmw_in_sb. }
+    desc.
+    assert (wf_thread_state thread state'') as GPC''.
+    { eapply wf_thread_state_steps; [|apply STEP1]; auto. }
+    exists state''. splits; auto.
+    edestruct steps_old_restrict with (state0:=state'') (state':=state') as [ORMW]; eauto.
+    desc. unnw.
+    constructor.
+    { rewrite CACTS. unfold CT, mkCT, G. 
+      rewrite E_E0; eauto. }
+    { ins. unfold G, rstG, restrict; simpls.
+      rewrite <- (tr_lab TEH); auto.
+      2: { eapply steps_preserve_E.
+           3: by apply EE.
+           all: eauto. }
+      assert (tid x = thread) as HH.
+      { apply GPC''.(acts_rep) in EE. desc. by subst. }
+      rewrite <- HH in *.
+      symmetry. eapply steps_preserve_lab; eauto. }
+    all: unfold G, rstG, restrict; simpls.
+    { rewrite ORMW. rewrite CACTS. unfold CT.
+      rewrite !seqA.
+      arewrite (⦗Tid_ thread⦘ ⨾ ⦗E0 Gf T S thread⦘ ⨾ rmw Gf ⨾ ⦗E0 Gf T S thread⦘ ⨾ ⦗Tid_ thread⦘ ≡
+                              ⦗E0 Gf T S thread⦘ ⨾ ⦗Tid_ thread⦘ ⨾ ⦗Tid_ thread⦘ ⨾ rmw Gf ⨾
+                              ⦗Tid_ thread⦘ ⨾ ⦗Tid_ thread⦘ ⨾ ⦗E0 Gf T S thread⦘).
       { basic_solver. }
-      edestruct (@sb_semi_total_l Gf r y w WF); auto.
-      { intros HH. apply (init_w WF) in HH.
-        clear -RR HH. type_solver. }
-      { by apply (rmw_in_sb WF). }
-      exfalso. eapply (wf_rmwi WF); eauto. }
-    { right. exists w. apply seq_eqv_r. split; [|split]; auto.
-      { right. by apply rmw_in_sb. }
-      apply (etc_I_in_S ETCCOH). apply AA. }
-    right. destruct AA as [y AA]. apply seq_eqv_r in AA. destruct AA as [AA BB].
-    exists y. apply seq_eqv_r. split; auto.
-    right. apply rewrite_trans_seq_cr_r.
-    { apply sb_trans. }
-    eexists; split; eauto. by apply rmw_in_sb. }
-  desc.
-  assert (wf_thread_state thread state'') as GPC''.
-  { eapply wf_thread_state_steps; [|apply STEP1]; auto. }
-  exists state''. splits; auto.
-  edestruct steps_old_restrict with (state0:=state'') (state':=state') as [ORMW]; eauto.
-  desc. unnw.
-  constructor.
-  { rewrite CACTS. unfold CT. rewrite H.
-    rewrite E_E0; eauto. }
-  { ins. rewrite H. unfold rstG, restrict; simpls.
-    rewrite <- (tr_lab TEH); auto.
-    2: { eapply steps_preserve_E.
-         3: by apply EE.
-         all: eauto. }
-    assert (tid x = thread) as HH.
-    { apply GPC''.(acts_rep) in EE. desc. by subst. }
-    rewrite <- HH in *.
-    symmetry. eapply steps_preserve_lab; eauto. }
-  all: rewrite H; unfold rstG, restrict; simpls.
-  { rewrite ORMW. rewrite CACTS. unfold CT.
+      seq_rewrite <- (tr_rmw TEH). unfold mkCT. basic_solver. }
+    { rewrite ODATA. rewrite CACTS. unfold CT.
+      rewrite !seqA.
+      arewrite (⦗Tid_ thread⦘ ⨾ ⦗E0 Gf T S thread⦘ ⨾ data Gf ⨾ ⦗E0 Gf T S thread⦘ ⨾ ⦗Tid_ thread⦘ ≡
+                              ⦗E0 Gf T S thread⦘ ⨾ ⦗Tid_ thread⦘ ⨾ ⦗Tid_ thread⦘ ⨾ data Gf ⨾
+                              ⦗Tid_ thread⦘ ⨾ ⦗Tid_ thread⦘ ⨾ ⦗E0 Gf T S thread⦘).
+      { basic_solver. }
+      seq_rewrite <- (tr_data TEH). unfold mkCT. basic_solver. }
+    { rewrite OADDR. rewrite CACTS. unfold CT.
+      rewrite !seqA.
+      arewrite (⦗Tid_ thread⦘ ⨾ ⦗E0 Gf T S thread⦘ ⨾ addr Gf ⨾ ⦗E0 Gf T S thread⦘ ⨾ ⦗Tid_ thread⦘ ≡
+                              ⦗E0 Gf T S thread⦘ ⨾ ⦗Tid_ thread⦘ ⨾ ⦗Tid_ thread⦘ ⨾ addr Gf ⨾
+                              ⦗Tid_ thread⦘ ⨾ ⦗Tid_ thread⦘ ⨾ ⦗E0 Gf T S thread⦘).
+      { basic_solver. }
+      seq_rewrite <- (tr_addr TEH). unfold mkCT. basic_solver. }
+    { rewrite OCTRL. rewrite CACTS. unfold CT.
+      rewrite !seqA.
+      arewrite (⦗Tid_ thread⦘ ⨾ ⦗E0 Gf T S thread⦘ ⨾ ctrl Gf ⨾ ⦗E0 Gf T S thread⦘ ⨾ ⦗Tid_ thread⦘ ≡
+                              ⦗E0 Gf T S thread⦘ ⨾ ⦗Tid_ thread⦘ ⨾ ⦗Tid_ thread⦘ ⨾ ctrl Gf ⨾
+                              ⦗Tid_ thread⦘ ⨾ ⦗Tid_ thread⦘ ⨾ ⦗E0 Gf T S thread⦘).
+      { basic_solver. }
+      seq_rewrite <- (tr_ctrl TEH). unfold mkCT. basic_solver. }
+    rewrite OFAILDEP. rewrite CACTS. unfold CT.
     rewrite !seqA.
-    arewrite (⦗Tid_ thread⦘ ⨾ ⦗E0 Gf T S thread⦘ ⨾ rmw Gf ⨾ ⦗E0 Gf T S thread⦘ ⨾ ⦗Tid_ thread⦘ ≡
-              ⦗E0 Gf T S thread⦘ ⨾ ⦗Tid_ thread⦘ ⨾ ⦗Tid_ thread⦘ ⨾ rmw Gf ⨾
-              ⦗Tid_ thread⦘ ⨾ ⦗Tid_ thread⦘ ⨾ ⦗E0 Gf T S thread⦘).
+    arewrite (⦗Tid_ thread⦘ ⨾ ⦗E0 Gf T S thread⦘ ⨾ rmw_dep Gf ⨾
+                            ⦗E0 Gf T S thread⦘ ⨾ ⦗Tid_ thread⦘ ≡
+                            ⦗E0 Gf T S thread⦘ ⨾ ⦗Tid_ thread⦘ ⨾ ⦗Tid_ thread⦘ ⨾ rmw_dep Gf ⨾
+                            ⦗Tid_ thread⦘ ⨾ ⦗Tid_ thread⦘ ⨾ ⦗E0 Gf T S thread⦘).
     { basic_solver. }
-    seq_rewrite <- (tr_rmw TEH). unfold mkCT. basic_solver. }
-  { rewrite ODATA. rewrite CACTS. unfold CT.
-    rewrite !seqA.
-    arewrite (⦗Tid_ thread⦘ ⨾ ⦗E0 Gf T S thread⦘ ⨾ data Gf ⨾ ⦗E0 Gf T S thread⦘ ⨾ ⦗Tid_ thread⦘ ≡
-              ⦗E0 Gf T S thread⦘ ⨾ ⦗Tid_ thread⦘ ⨾ ⦗Tid_ thread⦘ ⨾ data Gf ⨾
-              ⦗Tid_ thread⦘ ⨾ ⦗Tid_ thread⦘ ⨾ ⦗E0 Gf T S thread⦘).
-    { basic_solver. }
-    seq_rewrite <- (tr_data TEH). unfold mkCT. basic_solver. }
-  { rewrite OADDR. rewrite CACTS. unfold CT.
-    rewrite !seqA.
-    arewrite (⦗Tid_ thread⦘ ⨾ ⦗E0 Gf T S thread⦘ ⨾ addr Gf ⨾ ⦗E0 Gf T S thread⦘ ⨾ ⦗Tid_ thread⦘ ≡
-              ⦗E0 Gf T S thread⦘ ⨾ ⦗Tid_ thread⦘ ⨾ ⦗Tid_ thread⦘ ⨾ addr Gf ⨾
-              ⦗Tid_ thread⦘ ⨾ ⦗Tid_ thread⦘ ⨾ ⦗E0 Gf T S thread⦘).
-    { basic_solver. }
-    seq_rewrite <- (tr_addr TEH). unfold mkCT. basic_solver. }
-  { rewrite OCTRL. rewrite CACTS. unfold CT.
-    rewrite !seqA.
-    arewrite (⦗Tid_ thread⦘ ⨾ ⦗E0 Gf T S thread⦘ ⨾ ctrl Gf ⨾ ⦗E0 Gf T S thread⦘ ⨾ ⦗Tid_ thread⦘ ≡
-              ⦗E0 Gf T S thread⦘ ⨾ ⦗Tid_ thread⦘ ⨾ ⦗Tid_ thread⦘ ⨾ ctrl Gf ⨾
-              ⦗Tid_ thread⦘ ⨾ ⦗Tid_ thread⦘ ⨾ ⦗E0 Gf T S thread⦘).
-    { basic_solver. }
-    seq_rewrite <- (tr_ctrl TEH). unfold mkCT. basic_solver. }
-  rewrite OFAILDEP. rewrite CACTS. unfold CT.
-  rewrite !seqA.
-  arewrite (⦗Tid_ thread⦘ ⨾ ⦗E0 Gf T S thread⦘ ⨾ rmw_dep Gf ⨾
-                          ⦗E0 Gf T S thread⦘ ⨾ ⦗Tid_ thread⦘ ≡
-            ⦗E0 Gf T S thread⦘ ⨾ ⦗Tid_ thread⦘ ⨾ ⦗Tid_ thread⦘ ⨾ rmw_dep Gf ⨾
-            ⦗Tid_ thread⦘ ⨾ ⦗Tid_ thread⦘ ⨾ ⦗E0 Gf T S thread⦘).
-  { basic_solver. }
-  seq_rewrite <- (tr_rmw_dep TEH). unfold mkCT. basic_solver. }
-desc.
+    seq_rewrite <- (tr_rmw_dep TEH). unfold mkCT. basic_solver.
+  Qed.
 
-assert (acts_set (ProgToExecution.G state) ⊆₁ covered T) as STATECOV.
-{ intros x EE. apply (acts_rep GPC) in EE. desc. subst. by apply PCOV. }
+  Lemma COMP_RPPO:
+    dom_rel (⦗fun a => is_r (lab G) a⦘ ⨾ (data G ∪ rfi G ∪ rmw G)＊ ⨾ rppo G ⨾ ⦗S⦘)
+            ⊆₁ codom_rel (rf G).
+  Proof using WF SIMREL IMMCON.  subst. eapply COMP_RPPO; eauto. Qed. 
 
-assert (COMP_RPPO : dom_rel (⦗fun a => is_r (lab G) a⦘ ⨾ (data G ∪ rfi G ∪ rmw G)＊ ⨾ rppo G ⨾ ⦗S⦘)
-                        ⊆₁ codom_rel (rf G)).
-{ subst. eapply COMP_RPPO; edone. }
+  Lemma S_in_W: S ⊆₁ is_w (lab G).
+  Proof using WF SIMREL. 
+    rewrite (reservedW WF ETCCOH).
+    eapply sub_W; eauto. Qed.
+  
+  Lemma ST_in_E: S ∩₁ Tid_ thread ⊆₁ acts_set G.
+  Proof using WF SIMREL.
+    unfold G. rewrite E_E0; eauto. unfold E0.
+    unionR left -> right. basic_solver 10.
+  Qed.
+  
+  Lemma F_SB_S:
+    dom_rel (⦗(is_f (lab G)) ∩₁ (is_ra (lab G))⦘ ⨾ sb G ⨾ ⦗S⦘) ⊆₁ covered T.
+  Proof using WF SIMREL.
+    rewrite sub_F; eauto.
+    rewrite sub_AcqRel; eauto.
+    rewrite sub_sb_in; eauto.
+    apply ETCCOH.
+  Qed.
+  
+  Lemma RPPO_S:
+    dom_rel ((detour G ∪ rfe G) ⨾ (data G ∪ rfi G ∪ rmw G)＊ ⨾ rppo G ⨾ ⦗S⦘) ⊆₁ issued T.
+  Proof using WF SIMREL IMMCON.
+    rewrite sub_detour_in; eauto.
+    rewrite sub_rfe_in; eauto.
+    rewrite sub_data_in; eauto.
+    rewrite sub_rfi_in; eauto.
+    subst.
+    rewrite sub_rppo_in; eauto.
+    2: by eapply Frmw_E_prefix_clos; eauto.
+    rewrite sub_rmw_in; eauto.
+    apply ETCCOH.
+  Qed. 
 
-assert (S_in_W : S ⊆₁ is_w (lab G)).
-{ rewrite (reservedW WF ETCCOH).
-  eapply sub_W; eauto. }
-assert (ST_in_E : S ∩₁ Tid_ thread ⊆₁ acts_set G).
-{ subst. rewrite E_E0; eauto. unfold E0.
-  unionR left -> right. basic_solver 10. }
+  Lemma RMW_S: dom_rel ((detour G ∪ rfe G) ⨾ rmw G ⨾ ⦗S⦘) ⊆₁ issued T.
+  Proof using WF SIMREL. 
+    rewrite sub_detour_in; eauto.
+    rewrite sub_rfe_in; eauto.
+    rewrite sub_rmw_in; eauto.
+    eapply etc_rmw_S with (T:=mkETC T S); eauto.
+  Qed. 
+    
+  Lemma D_RMW_S: dom_rel (detour G ⨾ rmw G ⨾ ⦗S⦘) ⊆₁ issued T.
+  Proof using WF SIMREL. rewrite <- RMW_S. clear. basic_solver 10. Qed. 
 
-assert
-(F_SB_S :
-   dom_rel (⦗(is_f (lab G)) ∩₁ (is_ra (lab G))⦘ ⨾ sb G ⨾ ⦗S⦘) ⊆₁ covered T).
-{ rewrite sub_F; eauto.
-  rewrite sub_AcqRel; eauto.
-  rewrite sub_sb_in; eauto.
-  apply ETCCOH. }
-assert (RPPO_S : dom_rel ((detour G ∪ rfe G) ⨾ (data G ∪ rfi G ∪ rmw G)＊ ⨾ rppo G ⨾ ⦗S⦘) ⊆₁ issued T).
-{ rewrite sub_detour_in; eauto.
-  rewrite sub_rfe_in; eauto.
-  rewrite sub_data_in; eauto.
-  rewrite sub_rfi_in; eauto.
-  subst.
-  rewrite sub_rppo_in; eauto.
-  2: by eapply Frmw_E_prefix_clos; eauto.
-  rewrite sub_rmw_in; eauto.
-  apply ETCCOH. }
+  Lemma DRFE_RMW_RFI_R_ACQ:
+    dom_rel
+      ((detour G ∪ rfe G) ⨾ (rmw G ⨾ rfi G)＊ ⨾
+        ⦗(is_r (lab G)) ∩₁ (is_acq (lab G))⦘ ⨾ sb G ⨾ ⦗S⦘)
+      ⊆₁ issued T. 
+  Proof using WF SIMREL. 
+    rewrite sub_detour_in; eauto.
+    rewrite sub_rfe_in; eauto.
+    rewrite sub_rmw_in; eauto.
+    rewrite sub_rfi_in; eauto.
+    rewrite sub_R; eauto.
+    rewrite sub_Acq; eauto.
+    rewrite sub_sb_in; eauto.
+    apply ETCCOH.
+  Qed. 
 
-assert (RMW_S : dom_rel ((detour G ∪ rfe G) ⨾ rmw G ⨾ ⦗S⦘) ⊆₁ issued T).
-{ rewrite sub_detour_in; eauto.
-  rewrite sub_rfe_in; eauto.
-  rewrite sub_rmw_in; eauto.
-  eapply etc_rmw_S with (T:=mkETC T S); eauto. }
-assert (D_RMW_S : dom_rel (detour G ⨾ rmw G ⨾ ⦗S⦘) ⊆₁ issued T).
-{ rewrite <- RMW_S. clear. basic_solver 10. }
+  Hint Resolve COMP_RPPO S_in_W ST_in_E F_SB_S RPPO_S RMW_S D_RMW_S DRFE_RMW_RFI_R_ACQ: core.
 
-assert (dom_rel
-          ((detour G ∪ rfe G) ⨾ (rmw G ⨾ rfi G)＊ ⨾
-           ⦗(is_r (lab G)) ∩₁ (is_acq (lab G))⦘ ⨾ sb G ⨾ ⦗S⦘) ⊆₁ issued T)
-  as DRFE_RMW_RFI_R_ACQ.
-{ rewrite sub_detour_in; eauto.
-  rewrite sub_rfe_in; eauto.
-  rewrite sub_rmw_in; eauto.
-  rewrite sub_rfi_in; eauto.
-  rewrite sub_R; eauto.
-  rewrite sub_Acq; eauto.
-  rewrite sub_sb_in; eauto.
-  apply ETCCOH. }
+  Definition delta_rf :=
+    (new_rf G Gsc T S thread) ⨾ ⦗set_compl (dom_rel (rmw G))⦘ ∪
+    immediate (cert_co G T S thread) ⨾ (rmw G)⁻¹ ⨾ ⦗set_compl (D G T S thread)⦘.
+  Definition new_rfi := ⦗  Tid_ thread ⦘ ⨾ delta_rf ⨾ ⦗ Tid_ thread ⦘.
+  Definition new_rfe := ⦗ NTid_ thread ⦘ ⨾ delta_rf ⨾ ⦗ Tid_ thread ⦘.
 
-set (delta_rf :=
-       (new_rf G Gsc T S thread) ⨾ ⦗set_compl (dom_rel (rmw G))⦘ ∪
-       immediate (cert_co G T S thread) ⨾ (rmw G)⁻¹ ⨾ ⦗set_compl (D G T S thread)⦘).
-set (new_rfi := ⦗  Tid_ thread ⦘ ⨾ delta_rf ⨾ ⦗ Tid_ thread ⦘).
-set (new_rfe := ⦗ NTid_ thread ⦘ ⨾ delta_rf ⨾ ⦗ Tid_ thread ⦘).
+  Lemma DELTA_RF_CERT: delta_rf ⊆ cert_rf G Gsc T S thread.
+  Proof using. unfold delta_rf, cert_rf. basic_solver 20. Qed. 
 
-assert (delta_rf ⊆ cert_rf G Gsc T S thread) as DELTA_RF_CERT.
-{ unfold delta_rf, cert_rf; clear. basic_solver 20. }
+  Lemma delta_rfE:
+    delta_rf ≡ ⦗acts_set G⦘ ⨾ delta_rf ⨾ ⦗acts_set G \₁ D G T S thread⦘. 
+  Proof using WF SIMREL IMMCON. 
+    apply dom_helper_3.
+    arewrite (delta_rf ⊆ ⦗acts_set G⦘ ⨾ delta_rf ⨾ ⦗acts_set G⦘).
+    { apply dom_helper_3.
+      rewrite DELTA_RF_CERT. rewrite cert_rfE; eauto.
+      clear. basic_solver. }
+    unfold delta_rf. rewrite wf_new_rfE; auto.
+    basic_solver.
+  Qed.
 
-assert (delta_rf ≡
-        ⦗acts_set G⦘ ⨾ delta_rf ⨾ ⦗acts_set G \₁ D G T S thread⦘)
-  as delta_rfE.
-{ apply dom_helper_3.
-  arewrite (delta_rf ⊆ ⦗acts_set G⦘ ⨾ delta_rf ⨾ ⦗acts_set G⦘).
-  { apply dom_helper_3.
-    rewrite DELTA_RF_CERT. rewrite cert_rfE; eauto.
-    clear. basic_solver. }
-  subst delta_rf. rewrite wf_new_rfE; auto.
-  clear. basic_solver 30. }
+  Lemma delta_rfD:
+    delta_rf ≡ ⦗is_w (lab G)⦘ ⨾ delta_rf ⨾ ⦗is_r (lab G)⦘. 
+  Proof using WF SIMREL. 
+     apply dom_helper_3.
+     rewrite DELTA_RF_CERT. rewrite cert_rfD; auto. clear. basic_solver 10.
+  Qed. 
 
-assert (delta_rf ≡ ⦗is_w (lab G)⦘ ⨾ delta_rf ⨾ ⦗is_r (lab G)⦘)
-  as delta_rfD.
-{ apply dom_helper_3.
-  rewrite DELTA_RF_CERT. rewrite cert_rfD; auto. clear. basic_solver 10. }
+  Lemma NEW_RFI_CERT:
+    new_rfi ⊆ cert_rf G Gsc T S thread.
+  Proof using. unfold new_rfi. rewrite DELTA_RF_CERT. basic_solver 20. Qed. 
 
-assert (new_rfi ⊆ cert_rf G Gsc T S thread) as NEW_RFI_CERT.
-{ unfold new_rfi. rewrite DELTA_RF_CERT. basic_solver 20. }
-assert (new_rfif : functional new_rfi⁻¹).
-{ rewrite NEW_RFI_CERT. apply cert_rff; auto. }
+  Lemma new_rfif: functional new_rfi⁻¹. 
+  Proof using WF SIMREL IMMCON. rewrite NEW_RFI_CERT. apply cert_rff; auto. Qed.
 
-assert (new_rfe ⊆ cert_rf G Gsc T S thread) as NEW_RFE_CERT.
-{ unfold new_rfe. rewrite DELTA_RF_CERT. basic_solver 20. }
-assert (new_rfef : functional new_rfe⁻¹).
-{ rewrite NEW_RFE_CERT. apply cert_rff; auto. }
+  Lemma NEW_RFE_CERT: new_rfe ⊆ cert_rf G Gsc T S thread.
+  Proof using. unfold new_rfe. rewrite DELTA_RF_CERT. basic_solver 20. Qed.
 
-set (new_rfe_ex := new_rfe ∪ ⦗ set_compl (codom_rel new_rfe) ⦘).
+  Lemma new_rfef: functional new_rfe⁻¹. 
+  Proof using WF SIMREL IMMCON. rewrite NEW_RFE_CERT. apply cert_rff; auto. Qed.
 
-assert (new_rfe_unique: forall r, exists ! w, new_rfe_ex⁻¹  r w).
-{ ins.
-  destruct (classic ((codom_rel new_rfe) r)) as [X|X].
-  { unfolder in X; desf.
-    exists x; red; splits.
+  Hint Resolve delta_rfE delta_rfD NEW_RFE_CERT NEW_RFI_CERT new_rfif new_rfef: core. 
+
+  Definition new_rfe_ex := new_rfe ∪ ⦗ set_compl (codom_rel new_rfe) ⦘.
+
+  Lemma new_rfe_unique: forall r, exists ! w, new_rfe_ex⁻¹  r w. 
+  Proof using WF SIMREL IMMCON.
+    ins.
+    destruct (classic ((codom_rel new_rfe) r)) as [X|X].
+    { unfolder in X; desf.
+      exists x; red; splits.
+      unfold new_rfe_ex; basic_solver 12.
+      unfold new_rfe_ex; unfolder; ins; desf.
+      eapply new_rfef; basic_solver.
+      exfalso; eauto. }
+    exists r; red; splits.
     unfold new_rfe_ex; basic_solver 12.
     unfold new_rfe_ex; unfolder; ins; desf.
-    eapply new_rfef; basic_solver.
-    exfalso; eauto. }
-  exists r; red; splits.
-  unfold new_rfe_ex; basic_solver 12.
-  unfold new_rfe_ex; unfolder; ins; desf.
-  unfolder in X; exfalso; eauto. }
+    unfolder in X; exfalso; eauto.
+  Qed.
 
-assert (exists new_value, forall x, (new_rfe_ex)⁻¹ x (new_value x)); desc.
-{ apply (unique_choice (new_rfe_ex)⁻¹ (new_rfe_unique)). }
+  Hint Resolve new_rfe_unique: core. 
 
-set (get_val (v: option value) :=  match v with | Some v => v | _ => 0 end).
 
-set (new_val := fun r => get_val (val (lab G) (new_value r))).
+  Definition get_val (v: option value) :=  match v with | Some v => v | _ => 0 end.
 
-assert (ST_in_W_ex : S ∩₁ Tid_ thread \₁ issued T ⊆₁ W_ex G).
-{ arewrite (S ∩₁ Tid_ thread \₁ issued T ⊆₁
-            W_ex Gf ∩₁ S ∩₁ Tid_ thread \₁ issued T).
-  { unfolder. ins. desf. splits; auto.
-    apply (etc_S_I_in_W_ex ETCCOH). unfold eissued.
-    basic_solver. }
-  unfold W_ex.
-  rewrite (sub_rmw SUB).
-  subst.
-  unfolder. ins. desf.
-  eexists. splits; eauto.
-  all: eapply E_E0; eauto.
-  all: red.
-  all: left; right.
-  all: exists x; apply seq_eqv_r; split; [|split]; auto.
-  eapply inclusion_step_cr; [reflexivity|]. by apply (rmw_in_sb WF). }
+  Lemma ST_in_W_ex:
+    S ∩₁ Tid_ thread \₁ issued T ⊆₁ W_ex G.
+  Proof using WF SIMREL. 
+    arewrite (S ∩₁ Tid_ thread \₁ issued T ⊆₁
+                W_ex Gf ∩₁ S ∩₁ Tid_ thread \₁ issued T).
+    { unfolder. ins. desc. splits; auto.
+      apply (etc_S_I_in_W_ex ETCCOH). unfold eissued.
+      basic_solver. }
+    unfold W_ex.
+    rewrite (sub_rmw SUB).
+    subst.
+    unfolder. ins. desc.
+    eexists. splits; eauto.
+    all: eapply E_E0; eauto.
+    all: red.
+    all: left; right.
+    all: exists x; apply seq_eqv_r; split; [|split]; auto.
+    eapply inclusion_step_cr; [reflexivity|]. by apply (rmw_in_sb WF).
+  Qed.
 
-assert (SB_S : dom_sb_S_rfrmw G (mkETC T S) (rf G ⨾ ⦗R_ex (lab G)⦘) (issued T) ⊆₁ S).
-{ unfold dom_sb_S_rfrmw. 
-  rewrite sub_sb_in; eauto.
-  rewrite sub_rf_in; eauto.
-  rewrite sub_R_ex; eauto.
-  rewrite sub_rmw_in; eauto.
-  apply ETCCOH. }
-assert (RMWREX : dom_rel (rmw G) ⊆₁ (R_ex (lab G))).
-{ rewrite sub_rmw_in; eauto.
-  rewrite sub_R_ex; eauto.
-  apply COMMON. }
+  Lemma SB_S:
+    dom_sb_S_rfrmw G (mkETC T S) (rf G ⨾ ⦗R_ex (lab G)⦘) (issued T) ⊆₁ S.
+  Proof using WF SIMREL. 
+    unfold dom_sb_S_rfrmw. 
+    rewrite sub_sb_in; eauto.
+    rewrite sub_rf_in; eauto.
+    rewrite sub_R_ex; eauto.
+    rewrite sub_rmw_in; eauto.
+    apply ETCCOH.
+  Qed.
+  
+  Lemma RMWREX : dom_rel (rmw G) ⊆₁ (R_ex (lab G)).
+  Proof using SIMREL WF.
+    rewrite sub_rmw_in; eauto. rewrite sub_R_ex; eauto.
+    cdes SIMREL. apply COMMON.
+  Qed.
 
-assert (issued T ∪₁ S ∩₁ Tid_ thread ⊆₁ S) as IST_in_S.
-{ generalize (etc_I_in_S ETCCOH). unfold eissued. simpls.
-  basic_solver. } 
+  Lemma IST_in_S: issued T ∪₁ S ∩₁ Tid_ thread ⊆₁ S.
+  Proof using WF SIMREL. 
+    generalize (etc_I_in_S ETCCOH). unfold eissued. simpls.
+    basic_solver.
+  Qed.
 
-assert (issued T ⊆₁ S) as I_in_S by apply ETCCOH.
+  Lemma I_in_S: issued T ⊆₁ S.
+  Proof using WF SIMREL. by apply ETCCOH. Qed.
 
-exploit (@receptiveness_full thread state state'' new_val
-                               new_rfi (E0 Gf T S thread \₁ D G T S thread)); auto.
-{ clear -RMWRES. red in RMWRES. red. ins.
-  red. apply RMWRES in IN. red in IN. desf. }
-{ split; [|basic_solver].
-  rewrite TEH''.(tr_acts_set).
-  apply dom_helper_3.
-  rewrite set_interC at 2. unfold new_rfi.
-  rewrite delta_rfE. clear. basic_solver 10. }
-{ apply dom_helper_3.
-  unfold new_rfi. rewrite DELTA_RF_CERT.
-  rewrite cert_rfE; auto. rewrite !seqA.
-  rewrite cert_rfD; auto. rewrite !seqA.
-  seq_rewrite <- !id_inter.
-  rewrite set_interC with (s:=Tid_ thread) at 1.
-  rewrite <- TEH''.(tr_acts_set).
-  arewrite (acts_set (ProgToExecution.G state'') ∩₁  is_w (lab G) ≡₁
-            is_w (lab (ProgToExecution.G state'')) ∩₁
-            acts_set (ProgToExecution.G state'')).
-  { split.
-    all: intros x [AA BB]; split; auto.
-    all: unfold is_w in *; rewrite TEH''.(tr_lab) in *; auto. }
-  arewrite (is_r (lab G) ∩₁ acts_set (ProgToExecution.G state'') ≡₁
-            is_r (lab (ProgToExecution.G state'')) ∩₁
-            acts_set (ProgToExecution.G state'')).
-  { split.
-    all: intros x [AA BB]; split; auto.
-    all: unfold is_r in *; rewrite TEH''.(tr_lab) in *; auto. }
-  clear. basic_solver. }
-{ unfold new_rfi. rewrite DELTA_RF_CERT.
-  rewrite cert_rfE; auto. rewrite !seqA.
-  rewrite cert_rfD; auto. rewrite !seqA.
-  unfolder; ins; desc; subst thread.
-  apply (@same_thread G) in H5; try done.
-  2: { intro K; eapply init_w in K; try edone; type_solver. }
-  destruct H5 as [X|Y].
-  2: { unfold sb in Y; unfolder in Y; desf. }
-  destruct X; [subst; type_solver|]. 
-  exfalso.
-  eapply Cert_coherence.hb_rf_irr with (G:=G); eauto.
-  apply sb_in_hb in H1; unfolder; basic_solver 12. }
-{ unfold new_rfi. rewrite delta_rfE.
-  subst G; rewrite E_E0; try edone.
-  clear. basic_solver 10. }
-{ rewrite TEH''.(tr_acts_set).
-unfold D; subst G; rewrite E_E0; try edone.
-unfolder; ins; desf; splits; eauto.
-destruct (classic (tid x = thread)); try done.
-exfalso; apply H1; eauto 20. }
-{ rewrite STATECOV. rewrite C_in_D. basic_solver. }
-{ rewrite TEH''.(tr_rmw_dep).
-  arewrite_id ⦗Tid_ thread⦘; rels.
-  rewrite (@dom_frmw_in_D G _ _ S thread WF_G TCCOH_G); try done.
-  basic_solver. }
-{ rewrite TEH''.(tr_addr).
-  arewrite_id ⦗Tid_ thread⦘; rels.
-  rewrite (@dom_addr_in_D G _ _ S thread WF_G TCCOH_G); try done.
-  basic_solver. }
-{ rewrite TEH''.(tr_acts_set).
-  unfolder; ins; desc.
-  eapply H5; eauto.
-  eapply Rex_in_D with (sc:=Gsc) (T:=T); try done.
-  split; [|done].
-  unfold R_ex, rmwmod in *.
-  rewrite TEH''.(tr_lab) in H2; auto.
-  eapply TEH''.(tr_acts_set). by split. }
-{ rewrite TEH''.(tr_ctrl).
-  arewrite_id ⦗Tid_ thread⦘; rels.
-  rewrite (@dom_ctrl_in_D G _ _ S thread WF_G TCCOH_G); try done.
-  basic_solver. }
-{ rewrite TEH''.(tr_data).
-  rewrite (dom_r (wf_dataE WF_G)).
-  subst G.
-  rewrite (E_E0 thread WF ETCCOH).
-  unfolder; ins; desc.
-  eapply H4; splits; eauto.
-  intro.
-  apply H6.
-  apply (@dom_data_D (rstG Gf T S thread) Gsc T S thread WF_G); try done.
-  basic_solver 12. }
+  Hint Resolve ST_in_W_ex SB_S RMWREX IST_in_S I_in_S: core. 
+       
+  Definition receptiveness_def tid s_init s s'
+             (MOD: actid -> Prop) (new_val : actid -> value) :=
+    ⟪ STEPS' : (step tid)＊ s_init s' ⟫ /\
+    ⟪ RACTS : (acts_set (ProgToExecution.G s)) = (acts_set (ProgToExecution.G s')) ⟫ /\
+    ⟪ RRMW  : (rmw (ProgToExecution.G s))  ≡ (rmw (ProgToExecution.G s'))  ⟫ /\
+    ⟪ RDATA : (data (ProgToExecution.G s)) ≡ (data (ProgToExecution.G s')) ⟫ /\
+    ⟪ RADDR : (addr (ProgToExecution.G s)) ≡ (addr (ProgToExecution.G s')) ⟫ /\
+    ⟪ RCTRL : (ctrl (ProgToExecution.G s)) ≡ (ctrl (ProgToExecution.G s')) ⟫  /\
+    ⟪ RFAILRMW : (rmw_dep (ProgToExecution.G s)) ≡ (rmw_dep (ProgToExecution.G s')) ⟫  /\
+    ⟪ SAME : same_lab_u2v ((lab (ProgToExecution.G s'))) ((lab (ProgToExecution.G s)))⟫ /\
+    ⟪ NEW_VAL1 : forall r w (RF: new_rfi w r), val ((lab (ProgToExecution.G s'))) r = val ((lab (ProgToExecution.G s'))) w ⟫ /\
+    ⟪ NEW_VAL2 : forall r (RR : is_r (lab (ProgToExecution.G s')) r) (IN: MOD r) (NIN: ~ (codom_rel new_rfi) r),
+        val ((lab (ProgToExecution.G s'))) r = Some (new_val r) ⟫ /\
+    ⟪ OLD_VAL : forall a (NIN: ~ MOD a), val ((lab (ProgToExecution.G s'))) a = val ((lab (ProgToExecution.G s))) a ⟫.
 
-ins; desc. 
-set (lab' := fun x =>
-               if excluded_middle_informative ((ProgToExecution.G s').(acts_set) x) 
-               then s'.(ProgToExecution.G).(lab) x
-               else (lab G) x).
-assert (same_lab_u2v_dom (ProgToExecution.G s').(acts_set)
-                                 lab' (ProgToExecution.G s').(lab)) as SAME0.
-{ red. ins. red. unfold lab'. desf. }
+  Lemma receptiveness_impl state state'' (new_val: actid -> value)
+        (GPC: wf_thread_state thread state)
+        (RMWRES: RMWinstrProps.rmw_is_rex_instrs (instrs state))
+        (STEPS'': (step thread)＊ state state'')
+        (TEH'': thread_restricted_execution G thread (ProgToExecution.G state''))
+        (STATECOV : acts_set (ProgToExecution.G state) ⊆₁ covered T):
+    exists s', @receptiveness_def thread state state'' s' 
+                             (E0 Gf T S thread \₁ D G T S thread) new_val.
+  Proof using WF SIMREL IMMCON.
+    apply receptiveness_full; eauto.  
+    { red. ins. red. apply RMWRES in IN. red in IN. desf. }
+    { split; [|basic_solver].
+      rewrite TEH''.(tr_acts_set).
+      apply dom_helper_3.
+      rewrite set_interC at 2. unfold new_rfi.
+      rewrite delta_rfE. clear. basic_solver 10. }
+    { apply dom_helper_3.
+      unfold new_rfi. rewrite DELTA_RF_CERT.
+      rewrite cert_rfE; auto. rewrite !seqA.
+      rewrite cert_rfD; auto. rewrite !seqA.
+      seq_rewrite <- !id_inter.
+      rewrite set_interC with (s:=Tid_ thread) at 1.
+      rewrite <- TEH''.(tr_acts_set).
+      arewrite (acts_set (ProgToExecution.G state'') ∩₁  is_w (lab G) ≡₁
+                         is_w (lab (ProgToExecution.G state'')) ∩₁
+                         acts_set (ProgToExecution.G state'')).
+      { split.
+        all: intros x [AA BB]; split; auto.
+        all: unfold is_w in *; rewrite TEH''.(tr_lab) in *; auto. }
+      arewrite (is_r (lab G) ∩₁ acts_set (ProgToExecution.G state'') ≡₁
+                     is_r (lab (ProgToExecution.G state'')) ∩₁
+                     acts_set (ProgToExecution.G state'')).
+      { split.
+        all: intros x [AA BB]; split; auto.
+        all: unfold is_r in *; rewrite TEH''.(tr_lab) in *; auto. }
+      basic_solver. }
+    { unfold new_rfi. rewrite DELTA_RF_CERT.
+      rewrite cert_rfE; auto. rewrite !seqA.
+      rewrite cert_rfD; auto. rewrite !seqA.
+      repeat seq_rewrite <- id_inter. 
+      red. intros x y ?%seq_eqv_lr. unfold set_inter in *. desc. 
+      rewrite <- H0 in *.
+      apply (@same_thread G) in H4; try done.
+      2: { intro K; eapply init_w in K; try edone; type_solver. }
+      destruct H4 as [X|Y].
+      2: { unfold sb in Y; unfolder in Y; desf. }
+      destruct X; [subst; type_solver|]. 
+      exfalso.
+      rewrite -> H0 in *. 
+      eapply Cert_coherence.hb_rf_irr with (G:=G); eauto.
+      apply sb_in_hb in H; unfolder; basic_solver 12.
+      (* TODO: get rid of that *)
+      Unshelve. exact (fun _ => Afence Opln). }
+    { unfold new_rfi. rewrite delta_rfE.
+      unfold G; rewrite E_E0; basic_solver. }
+    { rewrite TEH''.(tr_acts_set).
+      unfold D, G; rewrite E_E0; try eauto.
+      unfolder; ins; desf; splits; eauto.
+      destruct (classic (tid x = thread)); try done.
+      exfalso; apply H0; eauto 20. }
+    { rewrite STATECOV. rewrite C_in_D. basic_solver. }
+    { rewrite TEH''.(tr_rmw_dep).
+      arewrite_id ⦗Tid_ thread⦘; rels.
+      rewrite (@dom_frmw_in_D G _ _ S thread WF_G TCCOH_G); try done.
+      basic_solver. }
+    { rewrite TEH''.(tr_addr).
+      arewrite_id ⦗Tid_ thread⦘; rels.
+      rewrite (@dom_addr_in_D G _ _ S thread WF_G TCCOH_G); try done.
+      basic_solver. }
+    { rewrite TEH''.(tr_acts_set).
+      unfolder; ins; desc.
+      eapply H3; eauto.
+      eapply Rex_in_D with (sc:=Gsc) (T:=T); try eauto.
+      split; [|done].
+      unfold R_ex, rmwmod in *.
+      rewrite TEH''.(tr_lab) in H0; auto.
+      eapply TEH''.(tr_acts_set). by split. }
+    { rewrite TEH''.(tr_ctrl).
+      arewrite_id ⦗Tid_ thread⦘; rels.
+      rewrite (@dom_ctrl_in_D G _ _ S thread WF_G TCCOH_G); try done.
+      basic_solver. }
+    { rewrite TEH''.(tr_data).
+      rewrite (dom_r (wf_dataE WF_G)).
+      unfold G.
+      rewrite (E_E0 thread WF ETCCOH).
+      unfolder; ins; desc.
+      eapply H3; splits; eauto.
+      intro.
+      apply H5.
+      apply (@dom_data_D (rstG Gf T S thread) Gsc T S thread WF_G); try done.
+      basic_solver 10. }
+  Qed.
 
-assert (same_lab_u2v_dom
-          (ProgToExecution.G s').(acts_set)
-          (ProgToExecution.G state'').(lab) (lab G)) as SAME2.
-{ rewrite <- RACTS.
-  apply same_lab_u2v_dom_comm.
-  eapply same_lab_u2v_dom_restricted; auto.
-  apply TEH''. }
-assert (same_lab_u2v_dom
-          (ProgToExecution.G s').(acts_set) lab' (lab G)) as SAME3.
-{ eapply same_lab_u2v_dom_trans; eauto.
-  eapply same_lab_u2v_dom_trans; eauto.
-    by apply same_lab_u2v_follows_set. }
+  Lemma XACQ_I: 
+    dom_rel (⦗W_ex G ∩₁ (is_xacq (lab G))⦘ ⨾ sb G ⨾ ⦗S⦘) ⊆₁ issued T.
+  Proof using WF SIMREL. 
+    rewrite sub_sb_in; eauto.
+    rewrite sub_xacq; eauto.
+    rewrite sub_W_ex_in; eauto.
+    apply ETCCOH.
+  Qed. 
 
-assert (same_lab_u2v lab' (lab G)) as SAME'.
-{ red. red. ins.
-  destruct (classic (acts_set (ProgToExecution.G s') e)) as [XX|XX].
-  { by apply SAME3. }
-  unfold lab'. desf. 
-  red. desf. }
+  Lemma COMP_RMW_S: dom_rel (rmw G ⨾ ⦗S⦘) ⊆₁ codom_rel (rf G).
+  Proof using WF SIMREL IMMCON. unfold G. eapply COMP_RMW_S; eauto. Qed.
 
-assert (thread_restricted_execution (certG G Gsc T S thread lab') thread
-                                    (ProgToExecution.G s')) as YY.
-{ constructor; auto.
-  { rewrite cert_E. rewrite <- RACTS. by rewrite TEH''.(tr_acts_set). }
-  { ins. unfold lab'. desf. }
-  all: unfold certG; simpls.
-  { rewrite <- RRMW. apply TEH''.(tr_rmw). }
-  { rewrite <- RDATA. apply TEH''.(tr_data). }
-  { rewrite <- RADDR. apply TEH''.(tr_addr). }
-  { rewrite <- RCTRL. apply TEH''.(tr_ctrl). }
-  rewrite <- RFAILRMW. apply TEH''.(tr_rmw_dep). }
+  Lemma RFRMW_IST_IN:
+    (cert_rf G Gsc T S thread ⨾ rmw G) ⨾ ⦗issued T ∪₁ S ∩₁ Tid_ thread⦘ ⊆ rf Gf ⨾ rmw Gf.
+  Proof using WF SIMREL IMMCON.  
+    rewrite IST_in_S. rewrite seqA.
+    rewrite cert_rmw_S_in_rf_rmw_S; auto using COMP_RMW_S. 
+    rewrite sub_rf_in; eauto.
+    rewrite sub_rmw_in; eauto.
+    basic_solver.
+  Qed. 
 
-assert (delta_rf ≡ new_rfi ∪ new_rfe) as NEWRF_SPLIT.
-{ arewrite (delta_rf ≡ delta_rf ⨾ ⦗ Tid_ thread ⦘).
-  2: { unfold new_rfi, new_rfe. 
-       rewrite <- seq_union_l. rewrite <- id_union.
-       arewrite (Tid_ thread ∪₁ NTid_ thread ≡₁ fun _ => True).
-       2: { clear. basic_solver. }
-       split; [basic_solver|].
-       intros x _. red. by destruct (classic (tid x = thread)); [left|right]. }
-  split; [|clear; basic_solver].
-  cut (codom_rel delta_rf ⊆₁ Tid_ thread).
-  { clear. basic_solver 21. }
-  rewrite delta_rfE at 1; try done.
-  unfold D.
-  unfolder; ins; desf.
-  destruct (classic (tid x = thread)); [done|].
-  exfalso; eapply H4. do 5 left. by right. }
+  Lemma RFRMW_IN: (cert_rf G Gsc T S thread ⨾ rmw G) ⨾ ⦗issued T⦘ ⊆ rf Gf ⨾ rmw Gf.
+  Proof using WF IMMCON SIMREL.
+    arewrite (issued T ⊆₁ issued T ∪₁ S ∩₁ Tid_ thread).
+    rewrite <- seqA. apply RFRMW_IST_IN. 
+  Qed. 
 
-assert (forall r w : actid, delta_rf w r -> val lab' w = val lab' r)
-  as SAME_VAL_RF.
-{ intros r w NEWRF.
-  apply NEWRF_SPLIT in NEWRF. destruct NEWRF as [NEWRF|NEWRF].
-  { set (VV := NEWRF). apply NEW_VAL1 in VV.
-    unfold new_rfi in NEWRF.
+  Lemma ISTex_rf_I:
+    (issued T ∪₁ S ∩₁ Tid_ thread) ∩₁ W_ex G ⊆₁
+    codom_rel (⦗issued T⦘ ⨾ rf G ⨾ rmw G).
+  Proof using WF SIMREL. 
+    assert ((issued T ∪₁ S ∩₁ Tid_ thread) ∩₁ W_ex G ⊆₁ S ∩₁ W_ex Gf) as AA.
+    { rewrite I_in_S. subst. unfold rstG, restrict, W_ex. simpls.
+      clear. basic_solver. }
+    intros x HH.
+    subst. unfold rstG, restrict, W_ex. simpls.
+    set (BB:=HH). apply AA in BB.
+    apply ETCCOH in BB. destruct BB as [y BB]. apply seq_eqv_l in BB.
+    destruct BB as [IY [z [BB CC]]].
+    exists y. apply seq_eqv_l. split; auto.
+    exists z.
+    assert (E0 Gf T S thread y) as E0Y.
+    { red. do 2 left. by right. }
+    assert (E0 Gf T S thread x) as E0X.
+    { destruct HH as [_ HH]. unfold rstG, restrict, W_ex in HH. simpls.
+      generalize HH. clear. basic_solver. }
+    assert (E0 Gf T S thread z) as E0Z.
+    2: by split; apply seq_eqv_lr; splits.
+    destruct HH as [DD HH].
+    assert (S x) as SX.
+    { destruct DD as [|DD]; [|by apply DD].
+        by apply (etc_I_in_S ETCCOH). }
+    destruct (classic (Tid_ thread x)) as [TID|NTID].
+    { red. left. right. exists x. apply seq_eqv_r. split.
+      2: by split.
+      right. by apply rmw_in_sb. }
+    destruct DD as [|DD]; eauto.
+    { right. exists x. apply seq_eqv_r. split; [|split]; auto. }
+    exfalso. apply NTID. apply DD.
+  Qed. 
+
+  Lemma DOM_SB_S_rf_I:
+    dom_rel (sb G ⨾ ⦗issued T ∪₁ S ∩₁ Tid_ thread⦘)
+            ∩₁ codom_rel (⦗issued T⦘ ⨾ rf G ⨾ ⦗R_ex (lab G)⦘ ⨾ rmw G) ⊆₁
+            issued T ∪₁ S ∩₁ Tid_ thread.
+  Proof using WF SIMREL. 
+    rewrite rmw_W_ex. rewrite (dom_r (wf_rmwE WF_G)).
+    rewrite <- !seqA. rewrite !codom_eqv1.
+    rewrite !seqA.
+
+    arewrite (R_ex (lab G) ⊆₁ R_ex (lab Gf)).
+    
+    rewrite sub_rf_in; eauto.
+    rewrite sub_rmw_in; eauto.
+    rewrite sub_sb_in; eauto.
+    arewrite (dom_rel (sb Gf ⨾ ⦗issued T ∪₁ S ∩₁ Tid_ thread⦘) ⊆₁
+                      dom_rel (sb Gf ⨾ ⦗issued T ∪₁ S ∩₁ Tid_ thread⦘) ∩₁
+                      dom_rel (sb Gf ⨾ ⦗S⦘)).
+    { generalize IST_in_S. clear. basic_solver 10. }
+    rewrite <- !set_interA. rewrite set_interC with (s':=W_ex G).
+    rewrite <- !set_interA. rewrite set_interC with (s':=acts_set G).
+    rewrite !set_interA.
+    
+    forward (eapply (etc_sb_S ETCCOH)); intro AA1.
+    unfold dom_sb_S_rfrmw in AA1.
+    simpl in AA1.
+    unfold eissued in AA1; simpl in AA1.
+    rewrite !seqA in AA1.
+    rewrite AA1.
+    rewrite <- !set_interA. rewrite (W_ex_in_W WF_G).
+    
+    simpls.
+    intros x [[HH AA] SX].
+    destruct (classic (issued T x)) as [|NISS]; [by left|].
+    destruct (classic (Tid_ thread x)) as [|NTID]; [by right; split|].
+    exfalso.
+    apply IT_new_co in HH. destruct HH as [HH|[_ HH]]; desf.
+  Qed. 
+
+  Hint Resolve XACQ_I COMP_RMW_S RFRMW_IST_IN RFRMW_IN ISTex_rf_I DOM_SB_S_rf_I: core. 
+
+  Section Lab'Properties.
+    Variable (s' state'': state).
+
+    Hypothesis TEH'':
+      thread_restricted_execution G thread (ProgToExecution.G state'').
+    Hypothesis (SAME: same_lab_u2v (lab (ProgToExecution.G s'))
+                                   (lab (ProgToExecution.G state''))). 
+
+
+    Variable (new_value: actid -> actid). 
+    Variable (st: state).
+
+    Definition new_val: actid -> value :=
+      fun (r: actid) => get_val (val (lab G) (new_value r)). 
+
+    Hypothesis     
+      (RECP: receptiveness_def thread st state'' s'
+                               (E0 Gf T S thread \₁ D G T S thread)
+                               new_val).
+
+    Hypothesis (H0: forall x, new_rfe_ex⁻¹ x (new_value x)). 
+    
+    Definition lab' :=
+      fun x =>
+        if excluded_middle_informative ((ProgToExecution.G s').(acts_set) x) 
+        then s'.(ProgToExecution.G).(lab) x
+        else (lab G) x.
+
+    Lemma SAME0: same_lab_u2v_dom (ProgToExecution.G s').(acts_set)
+                                  lab' (ProgToExecution.G s').(lab).
+    Proof using. red. ins. red. unfold lab'. desf. Qed. 
+
+    Lemma SAME2:
+      same_lab_u2v_dom (ProgToExecution.G s').(acts_set)
+          (ProgToExecution.G state'').(lab) (lab G).
+    Proof using TEH'' RECP.
+      cdes RECP. rewrite <- RACTS.
+      apply same_lab_u2v_dom_comm.
+      eapply same_lab_u2v_dom_restricted; auto.
+      apply TEH''.
+    Qed. 
+
+  Lemma SAME3:
+    same_lab_u2v_dom (ProgToExecution.G s').(acts_set) lab' (lab G).
+  Proof using TEH'' SAME RECP. 
+    eapply same_lab_u2v_dom_trans; eauto using SAME0. 
+    eapply same_lab_u2v_dom_trans; eauto using SAME2. 
+    by apply same_lab_u2v_follows_set.
+  Qed.
+
+  Lemma SAME':
+    same_lab_u2v lab' (lab G). 
+  Proof using TEH'' SAME RECP.
+    red. red. ins.
+    destruct (classic (acts_set (ProgToExecution.G s') e)) as [XX|XX].
+    { eapply SAME3; eauto. }
+    unfold lab'. desf. red. basic_solver.
+  Qed.
+
+  Lemma YY:
+    thread_restricted_execution (certG G Gsc T S thread lab') thread
+                                (ProgToExecution.G s').
+  Proof using TEH'' RECP.
+    cdes RECP.
+    constructor; auto.
+    { rewrite cert_E. rewrite <- RACTS. by rewrite TEH''.(tr_acts_set). }
+    { ins. unfold lab'. desf. }
+    all: unfold certG; simpls.
+    { rewrite <- RRMW. apply TEH''.(tr_rmw). }
+    { rewrite <- RDATA. apply TEH''.(tr_data). }
+    { rewrite <- RADDR. apply TEH''.(tr_addr). }
+    { rewrite <- RCTRL. apply TEH''.(tr_ctrl). }
+    { rewrite <- RFAILRMW. apply TEH''.(tr_rmw_dep). }
+  Qed. 
+
+  Lemma NEWRF_SPLIT: delta_rf ≡ new_rfi ∪ new_rfe.
+  Proof using WF SIMREL IMMCON.
+    arewrite (delta_rf ≡ delta_rf ⨾ ⦗ Tid_ thread ⦘).
+    2: { unfold new_rfi, new_rfe.
+         rewrite <- seq_union_l. rewrite <- id_union.
+         arewrite (Tid_ thread ∪₁ NTid_ thread ≡₁ fun _ => True).
+         2: { clear. basic_solver. }
+         split; [basic_solver|].
+         intros x _. red. by destruct (classic (tid x = thread)); [left|right]. }
+    split; [|clear; basic_solver].
+    cut (codom_rel delta_rf ⊆₁ Tid_ thread).
+    { clear. basic_solver 21. }
+    rewrite delta_rfE at 1; try done.
+    unfold D.
+    unfolder; ins; desf.
+    destruct (classic (tid x = thread)); [done|].
+    exfalso; eapply H3. do 5 left. by right.
+  Qed.
+
+  Lemma SAME_VAL_RF:
+    forall r w, delta_rf w r -> val lab' w = val lab' r.
+  Proof using WF SIMREL IMMCON TEH'' SAME RECP H0.
+    intros r w NEWRF. cdes RECP.
+    apply NEWRF_SPLIT in NEWRF. destruct NEWRF as [NEWRF|NEWRF].
+    { set (VV := NEWRF). apply NEW_VAL1 in VV.
+      unfold new_rfi in NEWRF.
+      apply seq_eqv_l in NEWRF. destruct NEWRF as [TIDW NEWRF].
+      apply seq_eqv_r in NEWRF. destruct NEWRF as [NEWRF TIDR].
+      apply delta_rfE in NEWRF; auto.
+      apply seq_eqv_l in NEWRF. destruct NEWRF as [GEW NEWRF].
+      apply seq_eqv_r in NEWRF. destruct NEWRF as [NEWRF [GER MOD]].
+      assert (s'.(ProgToExecution.G).(acts_set) r) as ERR.
+      { rewrite <- RACTS. apply TEH''.(tr_acts_set). split; auto. }
+      assert (s'.(ProgToExecution.G).(acts_set) w) as EWW.
+      { rewrite <- RACTS. apply TEH''.(tr_acts_set). split; auto. }
+      unfold lab', val.
+      destruct (excluded_middle_informative (acts_set (ProgToExecution.G s') w)) as [HH1|HH1].
+      2: by desf.
+      destruct (excluded_middle_informative (acts_set (ProgToExecution.G s') r)) as [HH2|HH2].
+      2: by desf.
+      symmetry. apply VV. }
+    assert (NEWRF0 := NEWRF).
+    unfold new_rfe in NEWRF.
     apply seq_eqv_l in NEWRF. destruct NEWRF as [TIDW NEWRF].
     apply seq_eqv_r in NEWRF. destruct NEWRF as [NEWRF TIDR].
     apply delta_rfE in NEWRF; auto.
     apply seq_eqv_l in NEWRF. destruct NEWRF as [GEW NEWRF].
     apply seq_eqv_r in NEWRF. destruct NEWRF as [NEWRF [GER MOD]].
-    assert (s'.(ProgToExecution.G).(acts_set) r) as ERR.
-    { rewrite <- RACTS. apply TEH''.(tr_acts_set). split; auto. }
-    assert (s'.(ProgToExecution.G).(acts_set) w) as EWW.
-    { rewrite <- RACTS. apply TEH''.(tr_acts_set). split; auto. }
-    unfold lab', val.
+    unfold val, lab'.
     destruct (excluded_middle_informative (acts_set (ProgToExecution.G s') w)) as [HH1|HH1].
-    2: by desf.
+    { exfalso. rewrite <- RACTS in HH1.
+      apply TEH''.(tr_acts_set) in HH1. destruct HH1 as [_ HH1]. desf. }
     destruct (excluded_middle_informative (acts_set (ProgToExecution.G s') r)) as [HH2|HH2].
+    2: { exfalso. apply HH2. rewrite <- RACTS. apply TEH''.(tr_acts_set).
+         split; auto. }
+    apply delta_rfD in NEWRF.
+    apply seq_eqv_l in NEWRF. destruct NEWRF as [WW NEWRF].
+    apply seq_eqv_r in NEWRF. destruct NEWRF as [NEWRF RR].
+    
+    assert (V: match lab (ProgToExecution.G s') r with
+               | Aload _ _ _ v | Astore _ _ _ v => Some v
+               | Afence _ => None
+               end = val (lab (ProgToExecution.G s')) r).
+    { by unfold val. }
+    rewrite V; erewrite NEW_VAL2.
+    { pose proof (new_rfe_unique r) as new_rfe_unique.
+      unfold unique in new_rfe_unique; desc.
+      specialize (H0 r).
+      assert (x = (new_value r)) by auto; subst x.
+      assert (NWW: new_value r =w).
+      { eapply new_rfe_unique0.
+          by unfold new_rfe_ex; basic_solver. }
+      subst w.
+      clear -WW.
+      unfold new_val, get_val.
+      unfold is_w, val in *. desf. }
+    { eapply same_lab_u2v_dom_is_r.
+      2: { split.
+           { apply HH2. }
+           eauto. }
+      eapply same_lab_u2v_dom_trans.
+      2: { eapply SAME2; eauto. }
+      red. ins. by apply SAME. }
+    { split; auto. unfold G in GER.
+      eapply E_E0 in GER; eauto. }
+    unfold new_rfi. intros [z NEWRFI].
+    apply seq_eqv_l in NEWRFI. destruct NEWRFI as [TIDZ NEWRFI].
+    apply seq_eqv_r in NEWRFI. destruct NEWRFI as [NEWRFI _].
+    assert (z = w) as XX.
     2: by desf.
-    symmetry. apply VV. }
-  assert (NEWRF0 := NEWRF).
-  unfold new_rfe in NEWRF.
-  apply seq_eqv_l in NEWRF. destruct NEWRF as [TIDW NEWRF].
-  apply seq_eqv_r in NEWRF. destruct NEWRF as [NEWRF TIDR].
-  apply delta_rfE in NEWRF; auto.
-  apply seq_eqv_l in NEWRF. destruct NEWRF as [GEW NEWRF].
-  apply seq_eqv_r in NEWRF. destruct NEWRF as [NEWRF [GER MOD]].
-  unfold val, lab'.
-  destruct (excluded_middle_informative (acts_set (ProgToExecution.G s') w)) as [HH1|HH1].
-  { exfalso. rewrite <- RACTS in HH1.
-    apply TEH''.(tr_acts_set) in HH1. destruct HH1 as [_ HH1]. desf. }
-  destruct (excluded_middle_informative (acts_set (ProgToExecution.G s') r)) as [HH2|HH2].
-  2: { exfalso. apply HH2. rewrite <- RACTS. apply TEH''.(tr_acts_set).
-       split; auto. }
-  apply delta_rfD in NEWRF.
-  apply seq_eqv_l in NEWRF. destruct NEWRF as [WW NEWRF].
-  apply seq_eqv_r in NEWRF. destruct NEWRF as [NEWRF RR].
+    eapply cert_rff.
+    4: { red; eauto. }
+    all: eauto.
+    all: eapply DELTA_RF_CERT; eauto.
+  Qed. 
 
-  assert (V: match lab (ProgToExecution.G s') r with
-             | Aload _ _ _ v | Astore _ _ _ v => Some v
-             | Afence _ => None
-             end = val (lab (ProgToExecution.G s')) r).
-  { by unfold val. }
-  rewrite V; erewrite NEW_VAL2.
-  { specialize (new_rfe_unique r).
-    unfold unique in new_rfe_unique; desc.
-    specialize (H0 r).
-    assert (x = (new_value r)) by auto; subst x.
-    assert (NWW: new_value r =w).
-    { eapply new_rfe_unique0.
-        by unfold new_rfe_ex; basic_solver. }
-    subst w.
-    clear -WW. 
-    unfold new_val, get_val.
-    unfold is_w, val in *. desf. }
-  { eapply same_lab_u2v_dom_is_r.
-    2: { split.
-         { apply HH2. }
-         eauto. }
-    eapply same_lab_u2v_dom_trans.
-    2: by apply SAME2.
-    red. ins. by apply SAME. }
-  { split; auto. rewrite H in GER.
-    eapply E_E0 in GER; eauto. }
-  unfold new_rfi. intros [z NEWRFI].
-  apply seq_eqv_l in NEWRFI. destruct NEWRFI as [TIDZ NEWRFI].
-  apply seq_eqv_r in NEWRFI. destruct NEWRFI as [NEWRFI _].
-  assert (z = w) as XX.
-  2: by desf.
-  eapply cert_rff.
-  4: { red; eauto. }
-  all: eauto.
-  all: eapply DELTA_RF_CERT; eauto. }
+  Lemma SAME_VAL:
+    forall a, ~ (acts_set G \₁ D G T S thread) a -> val lab' a = val (lab G) a.
+  Proof using WF SIMREL TEH'' RECP.
+    cdes RECP. 
+    intros a ZZ.
+    unfold val, lab'.
+    destruct (excluded_middle_informative (acts_set (ProgToExecution.G s') a)) as [MM|MM].
+    2: done.
+    assert (~ (E0 Gf T S thread \₁ D G T S thread) a) as XX.
+    { intros [AA BB]. apply ZZ. split; auto.
+      unfold G. eapply E_E0; eauto. }
+    specialize (OLD_VAL a XX). clear XX.
+    unfold val in OLD_VAL. rewrite OLD_VAL.
+    rewrite TEH''.(tr_lab); auto. by rewrite RACTS.
+  Qed.
 
-assert (forall a : actid, ~ (acts_set G \₁ D G T S thread) a -> val lab' a = val (lab G) a)
-  as SAME_VAL.
-{ intros a ZZ.
-  unfold val, lab'.
-  destruct (excluded_middle_informative (acts_set (ProgToExecution.G s') a)) as [MM|MM].
-  2: done.
-  assert (~ (E0 Gf T S thread \₁ D G T S thread) a) as XX.
-  { intros [AA BB]. apply ZZ. split; auto.
-    rewrite H. eapply E_E0; eauto. }
-  specialize (OLD_VAL a XX). clear XX.
-  unfold val in OLD_VAL. rewrite OLD_VAL.
-  rewrite TEH''.(tr_lab); auto. by rewrite RACTS. }
+  Lemma SAME_VAL_RF_CERT:
+    forall r w, (cert_rf G Gsc T S thread) w r -> val lab' w = val lab' r.
+  Proof using WF SIMREL IMMCON TEH'' SAME RECP H0.
+    intros r w HH. destruct HH as [[HH|HH]|HH].
+    2,3: eapply SAME_VAL_RF; eauto; unfold delta_rf; generalize HH.
+    2,3: clear; basic_solver 10.
+    erewrite !SAME_VAL; eauto. 
+    2,3: intros [_ AA]; apply AA.
+    3: { eapply dom_rf_D; eauto. eexists; eauto. }
+    2: { generalize HH. clear. basic_solver. }
+    apply wf_rfv; auto. generalize HH. basic_solver.
+  Qed. 
 
-assert (forall r w : actid, (cert_rf G Gsc T S thread) w r ->
-                            val lab' w = val lab' r)
-  as SAME_VAL_RF_CERT.
-{ intros r w HH. destruct HH as [[HH|HH]|HH].
-  2,3: apply SAME_VAL_RF; unfold delta_rf; generalize HH.
-  2,3: clear; basic_solver 10.
-  erewrite !SAME_VAL.
-  2,3: intros [_ AA]; apply AA.
-  3: { eapply dom_rf_D; eauto. eexists; eauto. }
-  2: { generalize HH. clear. basic_solver. }
-  apply wf_rfv; auto. generalize HH. clear. basic_solver. }
+  Lemma ISS_OLD: forall b (ISSB : issued T b), val lab' b = val (lab Gf) b.
+  Proof using TEH'' SIMREL RECP WF.
+    ins. rewrite <- lab_G_eq_lab_Gf.
+    rewrite SAME_VAL; auto.
+    intros [_ HH]. apply HH. by apply I_in_D.
+  Qed.
+  
+  Lemma acts_certG_in_acts_Gf:
+    acts_set (certG G Gsc T S thread lab') ⊆₁ acts_set Gf.
+  Proof using. unfold certG, G. simpl. basic_solver. Qed.
 
-assert (forall b (ISSB : issued T b), val lab' b = val (lab Gf) b) as ISS_OLD.
-{ ins. rewrite <- lab_G_eq_lab_Gf.
-  rewrite SAME_VAL; auto.
-  intros [_ HH]. apply HH. by apply I_in_D. }
+  Lemma WF_CERT: Wf (certG G Gsc T S thread lab'). 
+  Proof using WF TEH'' SIMREL SAME RECP IMMCON H0.
+    eapply WF_cert; eauto using SAME_VAL_RF_CERT, SAME_VAL, SAME'.
+  Qed.
 
-assert (acts_certG_in_acts_Gf : acts_set (certG G Gsc T S thread lab') ⊆₁ acts_set Gf).
-{ by unfold certG. }
+  Lemma WF_SC_CERT: wf_sc (certG G Gsc T S thread lab') Gsc.
+  Proof using WF TEH'' SIMREL SAME RECP IMMCON H0.
+    eapply WF_SC_cert; eauto using SAME'.
+  Qed.
 
-assert (dom_rel (⦗W_ex G ∩₁ (is_xacq (lab G))⦘ ⨾ sb G ⨾ ⦗S⦘) ⊆₁ issued T) as XACQ_I.
-{ rewrite sub_sb_in; eauto.
-  rewrite sub_xacq; eauto.
-  rewrite sub_W_ex_in; eauto.
-  apply ETCCOH. }
+  Hint Resolve SAME0 SAME2 SAME3 SAME' YY NEWRF_SPLIT SAME_VAL_RF SAME_VAL SAME_VAL_RF_CERT: core. 
+  Hint Resolve ISS_OLD acts_certG_in_acts_Gf WF_CERT WF_SC_CERT: core. 
 
-assert (dom_rel (rmw G ⨾ ⦗S⦘) ⊆₁ codom_rel (rf G)) as COMP_RMW_S.
-{ subst G. eapply COMP_RMW_S; eauto. }
+  End Lab'Properties.
 
-assert ((cert_rf G Gsc T S thread ⨾ rmw G) ⨾ ⦗issued T ∪₁ S ∩₁ Tid_ thread⦘ ⊆
-        rf Gf ⨾ rmw Gf) as RFRMW_IST_IN.
-{ rewrite IST_in_S. rewrite seqA.
-  rewrite cert_rmw_S_in_rf_rmw_S; auto.
-  rewrite sub_rf_in; eauto.
-  rewrite sub_rmw_in; eauto.
-  clear. basic_solver. }
+  Lemma FACQREL:
+    acts_set G ∩₁ (fun a : actid => is_f (lab G) a) ⊆₁ (fun a => is_ra (lab G) a).
+  Proof using SIMREL WF.
+    rewrite acts_G_in_acts_Gf.
+    rewrite lab_G_eq_lab_Gf. apply SIMREL.
+  Qed.
 
-assert ((cert_rf G Gsc T S thread ⨾ rmw G) ⨾ ⦗issued T⦘ ⊆ rf Gf ⨾ rmw Gf) as RFRMW_IN.
-{ arewrite (issued T ⊆₁ issued T ∪₁ S ∩₁ Tid_ thread). by rewrite <- seqA. }
+  Hint Resolve FACQREL: core. 
 
-assert (ISTex_rf_I :
-          (issued T ∪₁ S ∩₁ Tid_ thread) ∩₁ W_ex G ⊆₁ codom_rel (⦗issued T⦘ ⨾ rf G ⨾ rmw G)).
-{ assert ((issued T ∪₁ S ∩₁ Tid_ thread) ∩₁ W_ex G ⊆₁ S ∩₁ W_ex Gf) as AA.
-  { rewrite I_in_S. subst. unfold rstG, restrict, W_ex. simpls.
-    clear. basic_solver. }
-  intros x HH.
-  subst. unfold rstG, restrict, W_ex. simpls.
-  set (BB:=HH). apply AA in BB.
-  apply ETCCOH in BB. destruct BB as [y BB]. apply seq_eqv_l in BB.
-  destruct BB as [IY [z [BB CC]]].
-  exists y. apply seq_eqv_l. split; auto.
-  exists z.
-  assert (E0 Gf T S thread y) as E0Y.
-  { red. do 2 left. by right. }
-  assert (E0 Gf T S thread x) as E0X.
-  { destruct HH as [_ HH]. unfold rstG, restrict, W_ex in HH. simpls.
-    generalize HH. clear. basic_solver. }
-  assert (E0 Gf T S thread z) as E0Z.
-  2: by split; apply seq_eqv_lr; splits.
-  destruct HH as [DD HH].
-  assert (S x) as SX.
-  { destruct DD as [|DD]; [|by apply DD].
-      by apply (etc_I_in_S ETCCOH). }
-  destruct (classic (Tid_ thread x)) as [TID|NTID].
-  { red. left. right. exists x. apply seq_eqv_r. split.
-    2: by split.
-    right. by apply rmw_in_sb. }
-  destruct DD as [|DD]; eauto.
-  { right. exists x. apply seq_eqv_r. split; [|split]; auto. }
-  exfalso. apply NTID. apply DD. }
-assert (DOM_SB_S_rf_I :
-          dom_rel (sb G ⨾ ⦗issued T ∪₁ S ∩₁ Tid_ thread⦘)
-                  ∩₁ codom_rel (⦗issued T⦘ ⨾ rf G ⨾ ⦗R_ex (lab G)⦘ ⨾ rmw G) ⊆₁
-                  issued T ∪₁ S ∩₁ Tid_ thread).
-{ rewrite rmw_W_ex. rewrite (dom_r (wf_rmwE WF_G)).
-  rewrite <- !seqA. rewrite !codom_eqv1.
-  rewrite !seqA.
+  (* TODO: remove SAME hypothesis from the previous section *)
 
-  arewrite (R_ex (lab G) ⊆₁ R_ex (lab Gf)).
-  { subst G. unfold rstG, restrict. simpls. }
+  (* TODO: merge with Lab'Properties ? *)
+  Section SimRelCert.
+    Variable (state'' state s': ProgToExecution.state).
+    Variable (new_value: actid -> actid). 
+    Hypothesis (STEPS'' : (step thread)＊ state state''). 
+    Hypothesis (TEH'': thread_restricted_execution G thread (ProgToExecution.G state'')).
+    Hypothesis (NV: forall x, (new_rfe_ex)⁻¹ x (new_value x)). 
+    Hypothesis (RECP : receptiveness_def thread state state'' s'
+                                  (E0 Gf T S thread \₁ D G T S thread)
+                                  (new_val new_value)).
 
-  rewrite sub_rf_in; eauto.
-  rewrite sub_rmw_in; eauto.
-  rewrite sub_sb_in; eauto.
-  arewrite (dom_rel (sb Gf ⨾ ⦗issued T ∪₁ S ∩₁ Tid_ thread⦘) ⊆₁
-                    dom_rel (sb Gf ⨾ ⦗issued T ∪₁ S ∩₁ Tid_ thread⦘) ∩₁
-                    dom_rel (sb Gf ⨾ ⦗S⦘)).
-  { generalize IST_in_S. clear. basic_solver 10. }
-  rewrite <- !set_interA. rewrite set_interC with (s':=W_ex G).
-  rewrite <- !set_interA. rewrite set_interC with (s':=acts_set G).
-  rewrite !set_interA.
+    Lemma simrel_cert_common:
+      simrel_common (certG G Gsc T S thread (lab' s')) Gsc PC
+                    {| covered := covered T ∪₁ acts_set G ∩₁ NTid_ thread;
+                       issued := issued T |}
+                    (issued T ∪₁ S ∩₁ Tid_ thread) f_to f_from sim_certification.
+    Proof using WF TEH'' SIMREL RECP NV IMMCON FAIRf.
+      cdes SIMREL. cdes COMMON. cdes RECP.
+      (* TODO: eauto doesn't use hints? *)
+      red. splits; eauto; simpls; try by apply SIMREL.
+      { erewrite same_lab_u2v_is_rlx; eauto using SAME'.
+        rewrite <- cert_E. rewrite acts_G_in_acts_Gf; eauto. }
+      { erewrite same_lab_u2v_is_ra; eauto  using SAME'. 
+        rewrite <- cert_E, cert_F; eauto using SAME'. }
+      { eapply ETCCOH_cert; eauto using SAME_VAL_RF_CERT, SAME_VAL, WF_CERT, WF_SC_CERT, SAME'.  
+      }
+      { erewrite same_lab_u2v_is_rel; eauto using SAME'.
+        erewrite same_lab_u2v_is_w; eauto using SAME'.
+        rewrite RELCOV_G. basic_solver. }
+      { ins.
+        assert (acts_set G r) as ER.
+        { apply (dom_l (wf_rmwE WF_G)) in RMW. apply seq_eqv_l in RMW. desf. }
+        assert (acts_set G w) as EW.
+        { apply (dom_r (wf_rmwE WF_G)) in RMW. apply seq_eqv_r in RMW. desf. }
+        set (RMW' := RMW).
+        apply rmw_G_rmw_Gf in RMW'.
+        apply seq_eqv_l in RMW'. destruct RMW' as [EER RMW'].
+        apply seq_eqv_r in RMW'. destruct RMW' as [RMW' EEW].
+        assert (tid r = tid w) as TIDRW.
+        { by apply (wf_rmwt WF). }
+        split; (intros [COVV|[ACTS NTID]]; [by left; apply (RMWCOV r w)|]).
+        all: right; split; [auto|by generalize NTID; rewrite TIDRW]. }
+      { red. splits.
+        1,2: by (intros x [AA BB]; apply FCOH; split; auto).
+        { intros x HH AA. apply FCOH; auto. }
+        { ins. apply FCOH.
+          1,2: by apply IST_in_S.
+          assert ((cert_co G T S thread ⨾ ⦗cert_co_base G T S thread⦘) x y) as HH.
+          { apply seq_eqv_r. split; auto. apply IST_in_cert_co_base; auto. }
+          eapply cert_co_I in HH; eauto.
+          apply seq_eqv_r in HH. destruct HH as [HH _].
+          eapply (sub_co SUB) in HH.
+          apply seq_eqv_l in HH. destruct HH as [_ HH].
+          apply seq_eqv_r in HH. desf. }
+        ins. apply FCOH; auto.
+        apply RFRMW_IST_IN. apply seq_eqv_r. split; auto. }
+      { intros _.
+        erewrite same_lab_u2v_is_sc; eauto using SAME'.
+        erewrite same_lab_u2v_is_f; eauto using SAME'.
+        unfold certG, acts_set. simpls.
+        unfold G.
+        arewrite (acts_set (rstG Gf T S thread) ⊆₁ acts_set (rstG Gf T S thread)).
+        erewrite E_F_Sc_in_C; eauto.
+        basic_solver. }
+      { rewrite same_lab_u2v_R_ex; eauto  using SAME'. }
+      splits.
+      { unfold G.
+        erewrite <- cert_co_for_split with (G:=rstG Gf T S thread); eauto.
+        unfold cert_co_base.
+        hahn_frame. apply eqv_rel_mori.
+        apply AuxRel.set_compl_mori. red.
+          by erewrite Grfi_in_cert_rfi with (G:=rstG Gf T S thread); eauto. }
+      
+      unfold G. unfold W_ex. rewrite cert_sb. unfold certG. simpls.
+      rewrite <- seqA, codom_eqv1.
+      arewrite (codom_rel (⦗E0 Gf T S thread⦘ ⨾ rmw Gf) ⊆₁ is_w (lab Gf)).
+      { rewrite (wf_rmwD WF). basic_solver. }
+      (* TODO: introduce a lemma *)
+      arewrite (E0 Gf T S thread ⊆₁ E0 Gf T S thread ∩₁ E0 Gf T S thread).
+      rewrite <- set_interA.
+      unfold E0 at 1. rewrite !set_inter_union_r, !set_inter_union_l.
+      unionL.
+      4: { rewrite (wf_rmwD WF). type_solver 10. }
+      { rewrite w_covered_issued; eauto. basic_solver 10. }
+      { basic_solver 10. }
+      unfold sb. unfold rstG, restrict.
+      arewrite (Tid_ thread ∩₁ S ⊆₁ Tid_ thread ∩₁ S ∩₁ E0 Gf T S thread).
+      { assert (Tid_ thread ∩₁ S ⊆₁ E0 Gf T S thread) as AA.
+        { unfold E0. basic_solver 10. }
+        generalize AA. basic_solver. }
+      clear.
+      unfolder. ins. desf; eexists; eauto.
+      unfold acts_set; simpls. splits; [|by eauto].
+      right. splits; auto.
+      all: apply in_filterP_iff; splits; auto. 
+      Unshelve. all: done || exact (fun _ => Afence Opln).
+    Qed. 
+    
+    Lemma simrel_cert:
+      simrel_thread (certG G Gsc T S thread (lab' s')) Gsc PC
+                    {| covered := covered T ∪₁ acts_set G ∩₁ NTid_ thread;
+                       issued := issued T |}
+                    (issued T ∪₁ S ∩₁ Tid_ thread)
+                    f_to f_from thread sim_certification.
+    Proof.
+      red. splits.
+      { eapply simrel_cert_common; eauto. }
+      foobar. move existentials outside of simrel_*
+      
+      cdes SIMREL. red in  LOCAL. red in STATE. desc. cdes STATE0. 
+    
+red. splits.
+eexists. eexists. splits; eauto.
+(* { eapply GPC. } *)
+all: eauto.
+{ red. ins. eapply SIM_PROM in PROM. (* sim_prom *)
+  desc. exists b. splits; auto.
+  { unfold certG. unfold acts_set. simpls.
+    unfold G. unfold rstG, restrict. simpls. split; auto.
+    red. left. left. by right. }
+  { intros [HH|[_ HH]]; desf. }
+  { erewrite same_lab_u2v_loc; eauto.
+    rewrite <- lab_G_eq_lab_Gf. eapply SAME'; eauto. }
+  cdes HELPER.
+  red. splits; auto.
+  { unfold certG; simpls.
+    rewrite ISS_OLD; auto. }
+  intros ll. specialize (SIMMSG ll).
+  eapply max_value_same_set; eauto.
+  split; (intros x [AA|AA]; [left|right]).
+  4: { erewrite <- same_lab_u2v_loc in AA; eauto.
+       rewrite <- lab_G_eq_lab_Gf; eauto. }
+  2: { erewrite same_lab_u2v_loc in AA; eauto.
+       rewrite <- lab_G_eq_lab_Gf; eauto. }
+  { assert ((msg_rel Gf sc ll ⨾ ⦗ issued T ⦘) x b) as XX.
+    2: { apply seq_eqv_r in XX. desf. }
+    eapply msg_rel_I; eauto.
+    eapply cert_msg_rel with (lab':=lab'); eauto.
+    { by rewrite <- H. }
+    all: rewrite <- H; eauto.
+    all: try by unfold rst_sc; rewrite <- HeqGsc.
+    apply seq_eqv_r. split; auto.
+    unfold rst_sc. by rewrite <- HeqGsc. }
+  assert ((msg_rel (certG G Gsc T S thread lab') Gsc ll ⨾ ⦗ issued T ⦘) x b) as XX.
+  2: { apply seq_eqv_r in XX. desf. }
+  rewrite HeqGsc. rewrite H.
+  eapply cert_msg_rel; eauto.
+  all: rewrite <- H; auto.
+  all: try by rewrite <- HeqGsc; auto.
+  rewrite H.
+(*   eapply msg_rel_I; eauto. *)
+(*   apply seq_eqv_r. split; auto. } *)
+(* { red. ins. (* sim_res_prom *) *)
+(*   eapply SIM_RPROM in RES. *)
+(*   desc. *)
+(*   assert (acts_set Gf b) as FEB. *)
+(*   { by apply (etc_S_in_E ETCCOH). } *)
+(*   assert (acts_set G b) as EB. *)
+(*   { subst. eapply ST_in_E; eauto. by split. } *)
 
-  forward (eapply (etc_sb_S ETCCOH)); intro AA1.
-  unfold dom_sb_S_rfrmw in AA1.
-  simpl in AA1.
-  unfold eissued in AA1; simpl in AA1.
-  rewrite !seqA in AA1.
-  rewrite AA1.
-  rewrite <- !set_interA. rewrite (W_ex_in_W WF_G).
+(*   (* assert (~ issued T b /\ (S ∩₁ Tid_ thread) b) as [NIB SB]. *) *)
+(*   (* { apply seq_eqv_lr in RFRMWS. unfolder in RFRMWS. desf. } *) *)
+(*   (* set (AA:=RFRMWS). *) *)
+(*   (* apply seq_eqv_lr in AA. destruct AA as [_ [RFIRMW SB']]. *) *)
+(*   (* assert (~ is_init b) as NINITB. *) *)
+(*   (* { intros AA. apply NIB. eapply init_issued with (G:=Gf); eauto. *) *)
+(*   (*   split; auto. } *) *)
+(*   (* assert (same_tid b b') as STT. *) *)
+(*   (* { eapply (ninit_rfi_rmw_rt_same_tid WF). *) *)
+(*   (*   apply seq_eqv_l. by split. } *) *)
 
-  simpls.
-  intros x [[HH AA] SX].
-  destruct (classic (issued T x)) as [|NISS]; [by left|].
-  destruct (classic (Tid_ thread x)) as [|NTID]; [by right; split|].
-  exfalso.
-  apply IT_new_co in HH. destruct HH as [HH|[_ HH]]; desf. }
+(*   (* assert (acts_set G b') as EB'. *) *)
+(*   (* { subst. eapply ST_in_E; eauto. split; apply SB'. } *) *)
 
-exists (certG G Gsc T S thread lab').
-exists Gsc.
-exists (mkTC ((covered T) ∪₁ ((acts_set G) ∩₁ NTid_ thread)) (issued T)).
-exists ((issued T) ∪₁ S ∩₁ Tid_ thread).
+(*   (* destruct NOBEF as [w HH]. apply seq_eqv_l in HH. destruct HH as [IW RFRMW]. *) *)
+(*   (* destruct RFRMW as [r [RF RMW]]. *) *)
 
-assert (Wf (certG G Gsc T S thread lab')) as WF_CERT.
-{ eapply WF_cert; eauto. }
-assert (wf_sc (certG G Gsc T S thread lab') Gsc) as WF_SC_CERT.
-{ eapply WF_SC_cert; eauto. }
+(*   (* assert (acts_set G r) as ER. *) *)
+(*   (* { subst. eapply dom_sb_TS_in_E; eauto. *) *)
+(*   (*   exists b. apply seq_eqv_r. split. *) *)
+(*   (*   2: by split; apply SB. *) *)
+(*   (*   eapply inclusion_step_cr; [done|]. *) *)
+(*   (*     by apply (rmw_in_sb WF). } *) *)
 
-assert (acts_set G ∩₁ (fun a : actid => is_f (lab G) a) ⊆₁
-                 (fun a : actid => is_ra (lab G) a)) as FACQREL.
-{ rewrite acts_G_in_acts_Gf.
-  rewrite lab_G_eq_lab_Gf. apply SIMREL. }
+(*   (* assert (rmw G r b) as GRMW. *) *)
+(*   (* { subst. unfold rstG, restrict. simpls. *) *)
+(*   (*   apply seq_eqv_lr. splits; auto. *) *)
+(*   (*   all: eapply E_E0; eauto. } *) *)
+(*   (* assert (D G T S thread r) as DR. *) *)
+(*   (* { apply dom_rppo_S_in_D. exists b. *) *)
+(*   (*   apply seq_eqv_r. split; [|by apply SB]. *) *)
+(*   (*   apply rmw_in_rppo; auto. } *) *)
 
-splits; auto.
-{ apply cert_imm_consistent; auto. }
-{ unfold certG, acts_set; ins; basic_solver. }
-cdes SIMREL. cdes COMMON.
+(*   exists b. splits; auto. *)
+(*   { right. by split. } *)
+(*   erewrite same_lab_u2v_loc in LOC; eauto. *)
+(*   rewrite <- lab_G_eq_lab_Gf; eauto. *)
+(*     by apply same_lab_u2v_comm. } *)
+(* { red. ins. (* sim_mem *) *)
+(*   edestruct SIM_MEM with (b:=b) as [rel_opt]; eauto. *)
+(*   { erewrite same_lab_u2v_loc in LOC; eauto. *)
+(*     rewrite <- lab_G_eq_lab_Gf; eauto. } *)
+(*   { rewrite <- ISS_OLD; auto. apply VAL. } *)
+(*   simpls. desc. *)
+(*   exists rel_opt. *)
+(*   splits; eauto. *)
+(*   { red. cdes HELPER. splits; eauto. *)
+(*     intros ll. specialize (SIMMSG ll). *)
+(*     eapply max_value_same_set; eauto. *)
+(*     split; (intros x [AA|AA]; [left|right]). *)
+(*     4: { erewrite <- same_lab_u2v_loc in AA; eauto. *)
+(*          rewrite <- lab_G_eq_lab_Gf; eauto. } *)
+(*     2: { erewrite same_lab_u2v_loc in AA; eauto. *)
+(*          rewrite <- lab_G_eq_lab_Gf; eauto. } *)
+(*     { assert ((msg_rel Gf sc ll ⨾ ⦗ issued T ⦘) x b) as XX. *)
+(*       2: { apply seq_eqv_r in XX. desf. } *)
+(*       eapply msg_rel_I; eauto. *)
+(*       eapply cert_msg_rel with (lab':=lab'); eauto. *)
+(*       { by rewrite <- H. } *)
+(*       all: rewrite <- H; eauto. *)
+(*       all: try by unfold rst_sc; rewrite <- HeqGsc. *)
+(*       apply seq_eqv_r. split; auto. *)
+(*         by unfold rst_sc; rewrite <- HeqGsc. } *)
+(*     assert ((msg_rel (certG G Gsc T S thread lab') Gsc ll ⨾ ⦗ issued T ⦘) x b) as XX. *)
+(*     2: { apply seq_eqv_r in XX. desf. } *)
+(*     rewrite HeqGsc. rewrite H. *)
+(*     eapply cert_msg_rel; eauto. *)
+(*     all: rewrite <- H; auto. *)
+(*     all: try by rewrite <- HeqGsc; auto. *)
+(*     rewrite H. *)
+(*     eapply msg_rel_I; eauto. *)
+(*     apply seq_eqv_r. split; auto. } *)
+(*   rename H1 into UU. *)
+(*   intros UU1 UU2. *)
+(*   destruct UU as [AA BB]; auto. *)
+(*   { intros HH. apply UU2. by left. } *)
+(*   splits; auto. red in BB. desc. *)
+(*   exists p_rel. splits; auto. *)
+(*   destruct BB0; desc; [left|right]. *)
+(*   { split; auto. *)
+(*     intros HH. apply NINRMW. *)
+(*     destruct HH as [z HH]. apply seq_eqv_l in HH. desc. *)
+(*     exists z. apply seq_eqv_l. split; auto. *)
+(*     apply RFRMW_IN. apply seq_eqv_r. by split. } *)
+(*   exists p. splits; eauto. *)
+(*   { destruct INRMW as [z [RF RMW]]. *)
+(*     assert ((E0 Gf T S thread) z). *)
+(*     { unfold E0; left; right; exists b. *)
+(*       generalize (rmw_in_sb WF); basic_solver 12. } *)
+(*     assert ((E0 Gf T S thread) b). *)
+(*     { unfold E0; left; left; right; basic_solver 12. } *)
+(*     assert ((E0 Gf T S thread) p). *)
+(*     { unfold E0; left; left; right; basic_solver 12. } *)
+(*     assert ((rmw G) z b). *)
+(*     apply rmw_G_rmw_Gf; basic_solver 12. *)
+(*     exists z; splits; [|done]. *)
+(*     cut ((cert_rf G Gsc T S thread ⨾ ⦗D G T S thread⦘) p z). *)
+(*     { clear. basic_solver. } *)
+(*     apply cert_rf_D; auto. apply seq_eqv_r. split; auto. *)
+(*     { subst G. unfold rstG. unfold restrict. ins. *)
+(*       apply seq_eqv_lr. splits; auto. } *)
+(*     eapply dom_rmw_D; eauto. exists b. *)
+(*     apply seq_eqv_r. split; auto. by apply I_in_D. } *)
+(*   exists p_v. splits; eauto. *)
+(*   rewrite ISS_OLD; auto. } *)
+(* { red. ins. *)
+(*   assert (loc (lab Gf) b = Some l) as AA. *)
+(*   { rewrite <- LOC. symmetry. *)
+(*     erewrite same_lab_u2v_loc; eauto. *)
+(*       by rewrite <- lab_G_eq_lab_Gf. } *)
+(*   apply SIM_RES_MEM; auto. } *)
+(* { red. splits; red; ins. (* sim_tview *) *)
+(*   { assert *)
+(*       (t_cur (certG G Gsc T S thread lab') Gsc thread l *)
+(*              (covered T ∪₁ acts_set G ∩₁ NTid_ thread) ≡₁ *)
+(*              t_cur Gf sc thread l (covered T)) as XX. *)
+(*     2: { eapply max_value_same_set; eauto. apply SIM_TVIEW. } *)
+    
+(*     rewrite cert_t_cur_thread; try done. *)
+(*     arewrite (Gsc ≡ (rst_sc Gf sc T S thread)). *)
+(*     {  by unfold rst_sc; rewrite <- HeqGsc. } *)
+(*     subst; eapply t_cur_thread; try done. } *)
+
+(*   { assert *)
+(*       (t_acq (certG G Gsc T S thread lab') Gsc thread l *)
+(*              (covered T ∪₁ acts_set G ∩₁ NTid_ thread) ≡₁ *)
+(*              t_acq Gf sc thread l (covered T)) as XX. *)
+(*     2: { eapply max_value_same_set; eauto. apply SIM_TVIEW. } *)
+
+(*     rewrite cert_t_acq_thread; try done. *)
+(*     arewrite (Gsc ≡ (rst_sc Gf sc T S thread)). *)
+(*     { by unfold rst_sc; rewrite <- HeqGsc. } *)
+(*     subst; eapply t_acq_thread; try done. } *)
+
+(*   assert (t_rel (certG G Gsc T S thread lab') Gsc thread l l' *)
+(*                 (covered T ∪₁ acts_set G ∩₁ NTid_ thread) ≡₁ *)
+(*                 t_rel Gf sc thread l l' (covered T)) as XX. *)
+(*   { rewrite cert_t_rel_thread; try done. *)
+(*     arewrite (Gsc ≡ (rst_sc Gf sc T S thread)). *)
+(*     { by unfold rst_sc; rewrite <- HeqGsc. } *)
+(*     subst; eapply t_rel_thread; try done. } *)
+
+(*   cdes SIM_TVIEW. *)
+(*   eapply max_value_same_set. *)
+(*   { by apply REL. } *)
+(*   apply set_equiv_union; auto. *)
+(*   destruct (Loc.eq_dec l l'); [|done]. *)
+(*   erewrite same_lab_u2v_loc; eauto. *)
+(*   erewrite same_lab_u2v_is_w; eauto. *)
+(*   rewrite <- lab_G_eq_lab_Gf; eauto.  *)
+(*   unfold tid. basic_solver 10. } *)
+(* red. splits. (* sim_state *) *)
+(* { ins. split. *)
+(*   2: { intros HH. left. by apply PCOV. } *)
+(*   intros [HH|[_ HH]]; simpls. *)
+(*     by apply PCOV. } *)
+(* eexists. red. splits. *)
+(* { apply STEPS'. } *)
+(* { intros HH. inv HH. } *)
+(* done. *)
+(* Unshelve. *)
+(* all: clear.  *)
+(* all: exact (fun _ => Afence Orel) || exact (fun _ => True) || exact 0 || *)
+(*            exact (fun _ _ => True) || exact xH || *)
+(*            exact {| covered := ∅;  issued := ∅ |}. *)
+      Abort. 
+    
+    
+(* TODO: close section *)
+    
+Lemma cert_graph_init:
+    exists G' sc' T' S',
+      ⟪ WF : Wf G' ⟫ /\
+      ⟪ IMMCON : imm_consistent G' sc' ⟫ /\
+      ⟪ NTID  : NTid_ thread ∩₁ G'.(acts_set) ⊆₁ covered T' ⟫ /\
+      ⟪ SIMREL : simrel_thread G' sc' PC T' S' f_to f_from thread sim_certification ⟫.
+  Proof using All.
+    cdes SIMREL. cdes LOCAL.
+    red in STATE. desc.
+    cdes STATE0.
+    (* TODO: clean up context? *)
+   
+    assert (wf_thread_state thread state') as GPC'. 
+    { eapply wf_thread_state_steps. eauto. }
+
+    forward eapply CTINDEX; eauto. ins. desc. 
+    forward eapply STATE''; eauto. ins. desc. 
+    
+    assert (acts_set (ProgToExecution.G state) ⊆₁ covered T) as STATECOV.
+    { intros x EE. apply (acts_rep GPC) in EE. desc. subst. by apply PCOV. }
+
+    assert (exists new_value, forall x, (new_rfe_ex)⁻¹ x (new_value x)) as H0; desc.
+    { apply (unique_choice (new_rfe_ex)⁻¹ (new_rfe_unique)). }
+
+    set (new_val := new_val new_value). 
+    
+    forward eapply (@receptiveness_impl state state'' new_val); eauto.
+    intros RECP. desc. cdes RECP. 
+
+    forward eapply (@SAME0 s') as SAME0; eauto. 
+    forward eapply (@SAME2 s' state'') as SAME2; eauto. 
+    forward eapply (@SAME3 s' state'') as SAME3; eauto.
+    forward eapply (@SAME' s' state'') as SAME'; eauto.
+
+    forward eapply YY as YY; eauto.
+    
+    forward eapply NEWRF_SPLIT as NEWRF_SPLIT; eauto. 
+    pose proof (SAME_VAL_RF TEH'' SAME RECP H0) as SAME_VAL_RF. 
+    pose proof (SAME_VAL TEH'' RECP) as SAME_VAL. 
+    pose proof (SAME_VAL_RF_CERT TEH'' SAME RECP H0) as SAME_VAL_RF_CERT. 
+
+    exists (certG G Gsc T S thread (lab' s')).
+    exists Gsc.
+    exists (mkTC ((covered T) ∪₁ ((acts_set G) ∩₁ NTid_ thread)) (issued T)).
+    exists ((issued T) ∪₁ S ∩₁ Tid_ thread).
+
+    splits; eauto using WF_CERT. 
+    { eapply cert_imm_consistent; eauto using WF_CERT, WF_SC_CERT, FACQREL.
+      unfold G. by apply rstG_fair. }
+    { unfold certG, acts_set; ins; basic_solver. }
+
+
+    
+    cdes SIMREL. cdes COMMON.
 
 red. splits.
 { red. splits; eauto; simpls; try by apply SIMREL.
@@ -1288,5 +1853,8 @@ all: exact (fun _ => Afence Orel) || exact (fun _ => True) || exact 0 ||
            exact (fun _ _ => True) || exact xH ||
            exact {| covered := ∅;  issued := ∅ |}.
 Qed. 
+
+End CertGraphInit.
+
 
 End Cert.
